<?xml version="1.0"?>
<rdf:RDF xmlns="https://cogito.iot.linkeddata.es/platform#"
     xml:base="https://cogito.iot.linkeddata.es/platform"
     xmlns:dc="http://purl.org/dc/elements/1.1/"
     xmlns:owl="http://www.w3.org/2002/07/owl#"
     xmlns:rdf="http://www.w3.org/1999/02/22-rdf-syntax-ns#"
     xmlns:xml="http://www.w3.org/XML/1998/namespace"
     xmlns:xsd="http://www.w3.org/2001/XMLSchema#"
     xmlns:rdfs="http://www.w3.org/2000/01/rdf-schema#"
     xmlns:terms="http://purl.org/dc/terms/">
    <owl:Ontology rdf:about="https://cogito.iot.linkeddata.es/platform#">
        <dc:creator>María Poveda Villalón</dc:creator>
        <dc:creator>Raúl García Castro</dc:creator>
        <dc:creator>Socorro  Bernardos Galindo</dc:creator>
        <dc:description>The COGITO Platfrom ontology aims at modelling the entities considered in the the Digital Twin Platform, a component of the COGITO architecture</dc:description>
        <dc:title>Platform Ontology</dc:title>
        <terms:license rdf:resource="http://purl.org/NET/rdflicense/cc-by4.0"/>
        <owl:versionInfo>0.4.0</owl:versionInfo>
    </owl:Ontology>
    


    <!-- 
    ///////////////////////////////////////////////////////////////////////////////////////
    //
    // Annotation properties
    //
    ///////////////////////////////////////////////////////////////////////////////////////
     -->


    


    <!-- http://purl.org/dc/elements/1.1/creator -->


    <owl:AnnotationProperty rdf:about="http://purl.org/dc/elements/1.1/creator"/>
    


    <!-- http://purl.org/dc/elements/1.1/description -->


    <owl:AnnotationProperty rdf:about="http://purl.org/dc/elements/1.1/description"/>
    


    <!-- http://purl.org/dc/elements/1.1/title -->


    <owl:AnnotationProperty rdf:about="http://purl.org/dc/elements/1.1/title"/>
    


    <!-- http://purl.org/dc/terms/license -->


    <owl:AnnotationProperty rdf:about="http://purl.org/dc/terms/license"/>
    


    <!-- 
    ///////////////////////////////////////////////////////////////////////////////////////
    //
    // Object Properties
    //
    ///////////////////////////////////////////////////////////////////////////////////////
     -->


    


    <!-- https://cogito.iot.linkeddata.es/platform#hasFileFormat -->


    <owl:ObjectProperty rdf:about="https://cogito.iot.linkeddata.es/platform#hasFileFormat">
        <rdfs:subPropertyOf rdf:resource="https://www.w3.org/2019/wot/td#hasForm"/>
        <rdfs:comment>A sub-property of td:forms that relates a ctt:ConstructionTwinThing to a td:Form indicating its file format</rdfs:comment>
        <rdfs:label>has file format</rdfs:label>
    </owl:ObjectProperty>
    


    <!-- https://cogito.iot.linkeddata.es/platform#hasFileURL -->


    <owl:ObjectProperty rdf:about="https://cogito.iot.linkeddata.es/platform#hasFileURL">
        <rdfs:subPropertyOf rdf:resource="https://www.w3.org/2019/wot/td#hasForm"/>
        <rdfs:comment>A sub-property of td:forms that relates a ctt:ConstructionTwinThing to a td:Form indicating its file URL</rdfs:comment>
        <rdfs:label>has file URL</rdfs:label>
    </owl:ObjectProperty>
    


    <!-- https://cogito.iot.linkeddata.es/platform#hasIRI -->


    <owl:ObjectProperty rdf:about="https://cogito.iot.linkeddata.es/platform#hasIRI">
        <rdfs:subPropertyOf rdf:resource="https://www.w3.org/2019/wot/td#hasForm"/>
        <rdfs:comment>A sub-property of td:forms that relates a ctt:ConstructionTwinThing to a td:Form indicating its IRI</rdfs:comment>
        <rdfs:label>has IRI</rdfs:label>
    </owl:ObjectProperty>
    


    <!-- https://cogito.iot.linkeddata.es/platform#hasIfc -->


    <owl:ObjectProperty rdf:about="https://cogito.iot.linkeddata.es/platform#hasIfc">
        <rdfs:subPropertyOf rdf:resource="https://www.w3.org/2019/wot/td#hasLink"/>
        <rdfs:comment>A sub-property of td:links that relates a ctt:ConstructionTwinThing to a td:Link indicating its IFC file</rdfs:comment>
        <rdfs:label>has Ifc</rdfs:label>
    </owl:ObjectProperty>
    


    <!-- https://cogito.iot.linkeddata.es/platform#hasKnowledgeGraph -->


    <owl:ObjectProperty rdf:about="https://cogito.iot.linkeddata.es/platform#hasKnowledgeGraph">
        <rdfs:subPropertyOf rdf:resource="https://www.w3.org/2019/wot/td#hasForm"/>
        <rdfs:comment>A sub-property of td:forms that relates a ctt:ConstructionTwinThing to a td:Form indicating its knowledge graph</rdfs:comment>
        <rdfs:label>has knowledge graph</rdfs:label>
    </owl:ObjectProperty>
    


    <!-- https://cogito.iot.linkeddata.es/platform#hasMesh -->


    <owl:ObjectProperty rdf:about="https://cogito.iot.linkeddata.es/platform#hasMesh">
        <rdfs:subPropertyOf rdf:resource="https://www.w3.org/2019/wot/td#hasLink"/>
        <rdfs:comment>A sub-property of td:links that relates a ctt:ConstructionTwinThing to a td:Link indicating its mesh file</rdfs:comment>
        <rdfs:label>has mesh</rdfs:label>
    </owl:ObjectProperty>
    


    <!-- https://cogito.iot.linkeddata.es/platform#hasPointCloud -->


    <owl:ObjectProperty rdf:about="https://cogito.iot.linkeddata.es/platform#hasPointCloud">
        <rdfs:subPropertyOf rdf:resource="https://www.w3.org/2019/wot/td#hasLink"/>
        <rdfs:comment>A sub-property of td:links that relates a ctt:ConstructionTwinThing to a td:Link indicating its point cloud file</rdfs:comment>
        <rdfs:label>has point cloud</rdfs:label>
    </owl:ObjectProperty>
    


    <!-- https://cogito.iot.linkeddata.es/platform#hasSchedule -->


    <owl:ObjectProperty rdf:about="https://cogito.iot.linkeddata.es/platform#hasSchedule">
        <rdfs:subPropertyOf rdf:resource="https://www.w3.org/2019/wot/td#hasLink"/>
        <rdfs:comment>A sub-property of td:links that relates a ctt:ConstructionTwinThing to a td:Link indicating its schedule file</rdfs:comment>
        <rdfs:label>has schedule</rdfs:label>
    </owl:ObjectProperty>
    


    <!-- https://cogito.iot.linkeddata.es/platform#relatedTD -->


    <owl:ObjectProperty rdf:about="https://cogito.iot.linkeddata.es/platform#relatedTD">
        <rdfs:subPropertyOf rdf:resource="https://www.w3.org/2019/wot/td#hasLink"/>
        <rdfs:comment>A sub-property of td:links that relates a ctt:ConstructionTwinThing to a td:Link indicating a related thing description</rdfs:comment>
        <rdfs:label>related thing description</rdfs:label>
    </owl:ObjectProperty>
    


    <!-- https://www.w3.org/2019/wot/td#hasForm -->


    <owl:ObjectProperty rdf:about="https://www.w3.org/2019/wot/td#hasForm">
        <rdfs:range rdf:resource="https://www.w3.org/2019/wot/hypermedia#Form"/>
        <rdfs:isDefinedBy rdf:resource="https://www.w3.org/2019/wot/td#"/>
        <rdfs:label>has form</rdfs:label>
    </owl:ObjectProperty>
    


    <!-- https://www.w3.org/2019/wot/td#hasLink -->


    <owl:ObjectProperty rdf:about="https://www.w3.org/2019/wot/td#hasLink">
        <rdfs:range rdf:resource="https://www.w3.org/2019/wot/hypermedia#Link"/>
        <rdfs:isDefinedBy rdf:resource="https://www.w3.org/2019/wot/td#"/>
        <rdfs:label>has link</rdfs:label>
    </owl:ObjectProperty>
    


    <!-- 
    ///////////////////////////////////////////////////////////////////////////////////////
    //
    // Classes
    //
    ///////////////////////////////////////////////////////////////////////////////////////
     -->


    


    <!-- https://cogito.iot.linkeddata.es/def/facility#Element -->


    <owl:Class rdf:about="https://cogito.iot.linkeddata.es/def/facility#Element">
        <rdfs:subClassOf rdf:resource="https://cogito.iot.linkeddata.es/platform#DigitalTwin"/>
        <rdfs:comment>A subclass or bot:Element and, as such, a constituent of a construction entity with a characteristic technical function, form, or position</rdfs:comment>
        <rdfs:label>Element</rdfs:label>
    </owl:Class>
    


    <!-- https://cogito.iot.linkeddata.es/def/facility#Project -->


    <owl:Class rdf:about="https://cogito.iot.linkeddata.es/def/facility#Project">
        <rdfs:subClassOf rdf:resource="https://cogito.iot.linkeddata.es/platform#DigitalTwin"/>
        <rdfs:comment>A large or major undertaking, especially one involving considerable money, personnel, and equipment</rdfs:comment>
        <rdfs:label>Project</rdfs:label>
    </owl:Class>
    


    <!-- https://cogito.iot.linkeddata.es/platform#DigitalTwin -->


    <owl:Class rdf:about="https://cogito.iot.linkeddata.es/platform#DigitalTwin">
        <rdfs:subClassOf rdf:resource="https://cogito.iot.linkeddata.es/platform#PlanformThing"/>
        <rdfs:comment>Entity that is a digital twin in the platform</rdfs:comment>
        <rdfs:label>Digital Twin</rdfs:label>
    </owl:Class>
    


    <!-- https://cogito.iot.linkeddata.es/platform#PlanformThing -->


    <owl:Class rdf:about="https://cogito.iot.linkeddata.es/platform#PlanformThing">
        <rdfs:subClassOf rdf:resource="https://www.w3.org/2019/wot/td#Thing"/>
        <rdfs:comment>An entity that is a td:thing (entity whose metadata and interfaces are described by a WoT Thing Description) in the platform</rdfs:comment>
        <rdfs:label>Platform Thing</rdfs:label>
    </owl:Class>
    


    <!-- https://cogito.iot.linkeddata.es/quality#InformationResource -->


    <owl:Class rdf:about="https://cogito.iot.linkeddata.es/quality#InformationResource">
        <rdfs:subClassOf rdf:resource="https://cogito.iot.linkeddata.es/platform#PlanformThing"/>
        <rdfs:comment>Data regarding  the quality of an entity (especially a facility:Project or facility:Element) and that may have associated files in the platform</rdfs:comment>
        <rdfs:label>Information Resource</rdfs:label>
    </owl:Class>
    


    <!-- https://www.w3.org/2019/wot/hypermedia#Form -->


    <owl:Class rdf:about="https://www.w3.org/2019/wot/hypermedia#Form">
        <rdfs:label>Form</rdfs:label>
    </owl:Class>
    


    <!-- https://www.w3.org/2019/wot/hypermedia#Link -->


    <owl:Class rdf:about="https://www.w3.org/2019/wot/hypermedia#Link">
        <rdfs:label>Link</rdfs:label>
    </owl:Class>
    


    <!-- https://www.w3.org/2019/wot/td#Thing -->


    <owl:Class rdf:about="https://www.w3.org/2019/wot/td#Thing">
        <rdfs:isDefinedBy rdf:resource="https://www.w3.org/2019/wot/td#"/>
        <rdfs:label>Thing</rdfs:label>
    </owl:Class>
</rdf:RDF>



<!-- Generated by the OWL API (version 5.1.14) https://github.com/owlcs/owlapi/ -->


