@prefix : <https://cogito.iot.linkeddata.es/constwinthing#> .
@prefix owl: <http://www.w3.org/2002/07/owl#> .
@prefix rdf: <http://www.w3.org/1999/02/22-rdf-syntax-ns#> .
@prefix xml: <http://www.w3.org/XML/1998/namespace> .
@prefix xsd: <http://www.w3.org/2001/XMLSchema#> .
@prefix rdfs: <http://www.w3.org/2000/01/rdf-schema#> .
@base <https://cogito.iot.linkeddata.es/constwinthing#> .

<https://cogito.iot.linkeddata.es/constwinthing#> rdf:type owl:Ontology ;
                                                   <http://purl.org/dc/elements/1.1/creator> "María Poveda Villalón" ,
                                                                                             "Raúl García Castro" ,
                                                                                             "Socorro  Bernardos Galindo" ;
                                                   <http://purl.org/dc/elements/1.1/description> "The COGITO ConstructionTwin Thing ontology aims at modelling the (WoT) things considered in a construction twin." ;
                                                   <http://purl.org/dc/elements/1.1/title> "Construction Twin Thing Ontology" ;
                                                   <http://purl.org/dc/terms/license> <http://purl.org/NET/rdflicense/cc-by4.0> ;
                                                   owl:versionInfo "0.2.0" .

#################################################################
#    Annotation properties
#################################################################

###  http://purl.org/dc/elements/1.1/creator
<http://purl.org/dc/elements/1.1/creator> rdf:type owl:AnnotationProperty .


###  http://purl.org/dc/elements/1.1/description
<http://purl.org/dc/elements/1.1/description> rdf:type owl:AnnotationProperty .


###  http://purl.org/dc/elements/1.1/title
<http://purl.org/dc/elements/1.1/title> rdf:type owl:AnnotationProperty .


###  http://purl.org/dc/terms/license
<http://purl.org/dc/terms/license> rdf:type owl:AnnotationProperty .


#################################################################
#    Object Properties
#################################################################

###  https://cogito.iot.linkeddata.es/constwinthing#hasFile
:hasFile rdf:type owl:ObjectProperty ;
         rdfs:subPropertyOf <https://www.w3.org/2019/wot/td#forms> ;
         rdfs:comment "A sub-property of td:forms that relates a ctt:ConstructionTwinThing to a td:Form indicating its file" ;
         rdfs:label "has file" .


###  https://cogito.iot.linkeddata.es/constwinthing#hasIRI
:hasIRI rdf:type owl:ObjectProperty ;
        rdfs:subPropertyOf <https://www.w3.org/2019/wot/td#forms> ;
        rdfs:comment "A sub-property of td:forms that relates a ctt:ConstructionTwinThing to a td:Form indicating its IRI" ;
        rdfs:label "has IRI" .


###  https://cogito.iot.linkeddata.es/constwinthing#hasIfc
:hasIfc rdf:type owl:ObjectProperty ;
        rdfs:subPropertyOf <https://www.w3.org/2019/wot/td#links> ;
        rdfs:comment "A sub-property of td:links that relates a ctt:ConstructionTwinThing to a td:Link indicating its IFC file" ;
        rdfs:label "has Ifc" .


###  https://cogito.iot.linkeddata.es/constwinthing#hasKnowledgeGraph
:hasKnowledgeGraph rdf:type owl:ObjectProperty ;
                   rdfs:subPropertyOf <https://www.w3.org/2019/wot/td#forms> ;
                   rdfs:comment "A sub-property of td:forms that relates a ctt:ConstructionTwinThing to a td:Form indicating its knowledge graph" ;
                   rdfs:label "has knowledge graph" .


###  https://cogito.iot.linkeddata.es/constwinthing#hasMesh
:hasMesh rdf:type owl:ObjectProperty ;
         rdfs:subPropertyOf <https://www.w3.org/2019/wot/td#links> ;
         rdfs:comment "A sub-property of td:links that relates a ctt:ConstructionTwinThing to a td:Link indicating its mesh file" ;
         rdfs:label "has mesh" .


###  https://cogito.iot.linkeddata.es/constwinthing#hasPointCloud
:hasPointCloud rdf:type owl:ObjectProperty ;
               rdfs:subPropertyOf <https://www.w3.org/2019/wot/td#links> ;
               rdfs:comment "A sub-property of td:links that relates a ctt:ConstructionTwinThing to a td:Link indicating its point cloud file" ;
               rdfs:label "has point cloud" .


###  https://cogito.iot.linkeddata.es/constwinthing#hasSchedule
:hasSchedule rdf:type owl:ObjectProperty ;
             rdfs:subPropertyOf <https://www.w3.org/2019/wot/td#links> ;
             rdfs:comment "A sub-property of td:links that relates a ctt:ConstructionTwinThing to a td:Link indicating its schedule file" ;
             rdfs:label "has schedule" .


###  https://cogito.iot.linkeddata.es/constwinthing#relatedTD
:relatedTD rdf:type owl:ObjectProperty ;
           rdfs:subPropertyOf <https://www.w3.org/2019/wot/td#links> ;
           rdfs:comment "A sub-property of td:links that relates a ctt:ConstructionTwinThing to a td:Link indicating a related thing description" ;
           rdfs:label "related thing description" .


###  https://www.w3.org/2019/wot/td#forms
<https://www.w3.org/2019/wot/td#forms> rdf:type owl:ObjectProperty ;
                                       rdfs:range <https://www.w3.org/2019/wot/td#Form> ;
                                       rdfs:isDefinedBy <https://www.w3.org/2019/wot/td#> ;
                                       rdfs:label "forms" .


###  https://www.w3.org/2019/wot/td#links
<https://www.w3.org/2019/wot/td#links> rdf:type owl:ObjectProperty ;
                                       rdfs:range <https://www.w3.org/2019/wot/td#Link> ;
                                       rdfs:isDefinedBy <https://www.w3.org/2019/wot/td#> ;
                                       rdfs:label "links" .


#################################################################
#    Classes
#################################################################

###  https://cogito.iot.linkeddata.es/constwinthing#ConstructionTwinThing
:ConstructionTwinThing rdf:type owl:Class ;
                       rdfs:subClassOf <https://www.w3.org/2019/wot/td#Thing> ;
                       rdfs:comment "A subclass of a td:Thing and, as such, an abstraction of a physical or a virtual entity whose metadata and interfaces are described by a WoT Thing Description. In this case, an entity of a construction twin, namely, a facility:Project, a facility:Element, a qual:Image. a qual:PointCloud and a qual:Mesh." ;
                       rdfs:label "Construction Twin Thing" .


###  https://cogito.iot.linkeddata.es/def/facility#Element
<https://cogito.iot.linkeddata.es/def/facility#Element> rdf:type owl:Class ;
                                                        rdfs:subClassOf :ConstructionTwinThing ;
                                                        rdfs:comment "A subclass or bot:Element and, as such, a constituent of a construction entity with a characteristic technical function, form, or position" ;
                                                        rdfs:label "Element" .


###  https://cogito.iot.linkeddata.es/def/facility#Project
<https://cogito.iot.linkeddata.es/def/facility#Project> rdf:type owl:Class ;
                                                        rdfs:subClassOf :ConstructionTwinThing ;
                                                        rdfs:comment "A large or major undertaking, especially one involving considerable money, personnel, and equipment" ;
                                                        rdfs:label "Project" .


###  https://cogito.iot.linkeddata.es/quality#AsBuiltMesh
<https://cogito.iot.linkeddata.es/quality#AsBuiltMesh> rdf:type owl:Class ;
                                                       rdfs:subClassOf <https://cogito.iot.linkeddata.es/quality#Mesh> ;
                                                       rdfs:comment "A mesh representing a built entity (especially a facility:Element)" ;
                                                       rdfs:label "As-built Mesh" .


###  https://cogito.iot.linkeddata.es/quality#AsBuiltPointCloud
<https://cogito.iot.linkeddata.es/quality#AsBuiltPointCloud> rdf:type owl:Class ;
                                                             rdfs:subClassOf <https://cogito.iot.linkeddata.es/quality#PointCoud> ;
                                                             rdfs:comment "A point cloud representing a built entity (especially a facility:Element)" ;
                                                             rdfs:label "As-built Point Cloud" .


###  https://cogito.iot.linkeddata.es/quality#Image
<https://cogito.iot.linkeddata.es/quality#Image> rdf:type owl:Class ;
                                                 rdfs:subClassOf :ConstructionTwinThing ;
                                                 rdfs:comment "A picture of an entity" ;
                                                 rdfs:label "Image" .


###  https://cogito.iot.linkeddata.es/quality#Mesh
<https://cogito.iot.linkeddata.es/quality#Mesh> rdf:type owl:Class ;
                                                rdfs:subClassOf :ConstructionTwinThing ;
                                                rdfs:comment "A collection of vertices, edges and faces that defines the shape of an object (especially a facility:Element)" ;
                                                rdfs:label "Mesh" .


###  https://cogito.iot.linkeddata.es/quality#PointCoud
<https://cogito.iot.linkeddata.es/quality#PointCoud> rdf:type owl:Class ;
                                                     rdfs:subClassOf :ConstructionTwinThing ;
                                                     rdfs:comment "A set of data points in space" ;
                                                     rdfs:label "Point Cloud" .


###  https://cogito.iot.linkeddata.es/quality#RawImage
<https://cogito.iot.linkeddata.es/quality#RawImage> rdf:type owl:Class ;
                                                    rdfs:subClassOf <https://cogito.iot.linkeddata.es/quality#Image> ;
                                                    rdfs:comment "An image that has not been processed" ;
                                                    rdfs:label "Raw Image" .


###  https://www.w3.org/2019/wot/td#Form
<https://www.w3.org/2019/wot/td#Form> rdf:type owl:Class ;
                                      rdfs:isDefinedBy <https://www.w3.org/2019/wot/td#> ;
                                      rdfs:label "Form" .


###  https://www.w3.org/2019/wot/td#Link
<https://www.w3.org/2019/wot/td#Link> rdf:type owl:Class ;
                                      rdfs:isDefinedBy <https://www.w3.org/2019/wot/td#> ;
                                      rdfs:label "Link" .


###  https://www.w3.org/2019/wot/td#Thing
<https://www.w3.org/2019/wot/td#Thing> rdf:type owl:Class ;
                                       rdfs:isDefinedBy <https://www.w3.org/2019/wot/td#> ;
                                       rdfs:label "Thing" .


###  Generated by the OWL API (version 5.1.14) https://github.com/owlcs/owlapi/
