<?xml version="1.0"?>
<rdf:RDF xmlns="https://cogito.iot.linkeddata.es/quality#"
     xml:base="https://cogito.iot.linkeddata.es/quality"
     xmlns:dc="http://purl.org/dc/elements/1.1/"
     xmlns:owl="http://www.w3.org/2002/07/owl#"
     xmlns:rdf="http://www.w3.org/1999/02/22-rdf-syntax-ns#"
     xmlns:xml="http://www.w3.org/XML/1998/namespace"
     xmlns:xsd="http://www.w3.org/2001/XMLSchema#"
     xmlns:rdfs="http://www.w3.org/2000/01/rdf-schema#"
     xmlns:terms="http://purl.org/dc/terms/">
    <owl:Ontology rdf:about="https://cogito.iot.linkeddata.es/quality#">
        <dc:creator>María Poveda Villalón</dc:creator>
        <dc:creator>Raúl García Castro</dc:creator>
        <dc:creator>Socorro  Bernardos Galindo</dc:creator>
        <dc:description>The COGITO Quality ontology aims at modelling the construction quality domain.</dc:description>
        <dc:title>Quality Ontology</dc:title>
        <terms:license rdf:resource="http://purl.org/NET/rdflicense/cc-by4.0"/>
        <owl:versionInfo>0.9.0</owl:versionInfo>
    </owl:Ontology>
    


    <!-- 
    ///////////////////////////////////////////////////////////////////////////////////////
    //
    // Annotation properties
    //
    ///////////////////////////////////////////////////////////////////////////////////////
     -->


    


    <!-- http://purl.org/dc/elements/1.1/creator -->


    <owl:AnnotationProperty rdf:about="http://purl.org/dc/elements/1.1/creator"/>
    


    <!-- http://purl.org/dc/elements/1.1/description -->


    <owl:AnnotationProperty rdf:about="http://purl.org/dc/elements/1.1/description"/>
    


    <!-- http://purl.org/dc/elements/1.1/title -->


    <owl:AnnotationProperty rdf:about="http://purl.org/dc/elements/1.1/title"/>
    


    <!-- http://purl.org/dc/terms/license -->


    <owl:AnnotationProperty rdf:about="http://purl.org/dc/terms/license"/>
    


    <!-- 
    ///////////////////////////////////////////////////////////////////////////////////////
    //
    // Object Properties
    //
    ///////////////////////////////////////////////////////////////////////////////////////
     -->


    


    <!-- https://cogito.iot.linkeddata.es/def/quality#isRelatedToProject -->


    <owl:ObjectProperty rdf:about="https://cogito.iot.linkeddata.es/def/quality#isRelatedToProject">
        <rdfs:range rdf:resource="https://cogito.iot.linkeddata.es/def/facility#Project"/>
        <rdfs:comment>Property that relates an entity (especially qual:QualityInformation and quel:Rule) to a facility:Project</rdfs:comment>
        <rdfs:label>is related to project</rdfs:label>
    </owl:ObjectProperty>
    


    <!-- https://cogito.iot.linkeddata.es/quality#hasProcessedImage -->


    <owl:ObjectProperty rdf:about="https://cogito.iot.linkeddata.es/quality#hasProcessedImage">
        <rdfs:range rdf:resource="https://cogito.iot.linkeddata.es/quality#Image"/>
        <rdfs:comment>Property that relates an entity (especially qual:ImageJob to a processed qual:Image</rdfs:comment>
        <rdfs:label>has processed image</rdfs:label>
    </owl:ObjectProperty>
    


    <!-- https://cogito.iot.linkeddata.es/quality#hasRawImage -->


    <owl:ObjectProperty rdf:about="https://cogito.iot.linkeddata.es/quality#hasRawImage">
        <rdfs:subPropertyOf rdf:resource="http://www.w3.org/2002/07/owl#topObjectProperty"/>
        <rdfs:range rdf:resource="https://cogito.iot.linkeddata.es/quality#RawImage"/>
        <rdfs:comment>Property that relates an entity (especially qual:ImageJob to an original qual:Image</rdfs:comment>
        <rdfs:label>has raw image</rdfs:label>
    </owl:ObjectProperty>
    


    <!-- https://cogito.iot.linkeddata.es/quality#hasResultImage -->


    <owl:ObjectProperty rdf:about="https://cogito.iot.linkeddata.es/quality#hasResultImage">
        <rdfs:range rdf:resource="https://cogito.iot.linkeddata.es/quality#Image"/>
        <rdfs:comment>Property that relates an entity (especially qual:ImageJob to a resulting qual:Image</rdfs:comment>
        <rdfs:label>has result image</rdfs:label>
    </owl:ObjectProperty>
    


    <!-- https://cogito.iot.linkeddata.es/quality#isRelatedToElement -->


    <owl:ObjectProperty rdf:about="https://cogito.iot.linkeddata.es/quality#isRelatedToElement">
        <rdfs:range rdf:resource="https://cogito.iot.linkeddata.es/def/facility#Element"/>
        <rdfs:comment>Property that relates an entity (especially qual:QualityInformation) to a facility:Element</rdfs:comment>
        <rdfs:label>is related to element</rdfs:label>
    </owl:ObjectProperty>
    


    <!-- https://cogito.iot.linkeddata.es/quality#isRelatedToWorkOrder -->


    <owl:ObjectProperty rdf:about="https://cogito.iot.linkeddata.es/quality#isRelatedToWorkOrder">
        <rdfs:range rdf:resource="https://cogito.iot.linkeddata.es/process#WorkOrder"/>
        <rdfs:comment>Property that relates an entity (especially qual:QuqlityInformation) to a process:WorkOrder</rdfs:comment>
        <rdfs:label>is related to work order</rdfs:label>
    </owl:ObjectProperty>
    


    <!-- https://cogito.iot.linkeddata.es/quality#refelctsQualityResult -->


    <owl:ObjectProperty rdf:about="https://cogito.iot.linkeddata.es/quality#refelctsQualityResult">
        <rdfs:comment>Property that relates an entity (especially qual:QuqlityInformation to a qual:QualityResult</rdfs:comment>
        <rdfs:label>reflects quality result</rdfs:label>
    </owl:ObjectProperty>
    


    <!-- https://cogito.iot.linkeddata.es/quality#refersToElement -->


    <owl:ObjectProperty rdf:about="https://cogito.iot.linkeddata.es/quality#refersToElement">
        <rdfs:range rdf:resource="https://cogito.iot.linkeddata.es/def/facility#Element"/>
        <rdfs:comment>Property that relates an entity (especially qual:QualityResult) to a facility:Element</rdfs:comment>
        <rdfs:label>refers to element</rdfs:label>
    </owl:ObjectProperty>
    


    <!-- https://cogito.iot.linkeddata.es/quality#refersToRule -->


    <owl:ObjectProperty rdf:about="https://cogito.iot.linkeddata.es/quality#refersToRule">
        <rdfs:range rdf:resource="https://cogito.iot.linkeddata.es/quality#Rule"/>
        <rdfs:comment>Property that relates an entity (especially qual:Defect) to a qual:Rule</rdfs:comment>
        <rdfs:label>refers to rule</rdfs:label>
    </owl:ObjectProperty>
    


    <!-- https://cogito.iot.linkeddata.es/quality#reflectsDefect -->


    <owl:ObjectProperty rdf:about="https://cogito.iot.linkeddata.es/quality#reflectsDefect">
        <rdfs:subPropertyOf rdf:resource="https://cogito.iot.linkeddata.es/quality#refelctsQualityResult"/>
        <rdfs:range rdf:resource="https://cogito.iot.linkeddata.es/quality#Defect"/>
        <rdfs:comment>Property that relates an entity (especially qual:ImageJob) to a qual:Defect</rdfs:comment>
        <rdfs:label>reflects defect</rdfs:label>
    </owl:ObjectProperty>
    


    <!-- https://cogito.iot.linkeddata.es/quality#reflectsGeometricQuality -->


    <owl:ObjectProperty rdf:about="https://cogito.iot.linkeddata.es/quality#reflectsGeometricQuality">
        <rdfs:subPropertyOf rdf:resource="https://cogito.iot.linkeddata.es/quality#refelctsQualityResult"/>
        <rdfs:range rdf:resource="https://cogito.iot.linkeddata.es/quality#GeometricQualityInformation"/>
        <rdfs:comment>Property that relates an entity (especially qual:PointCloud) to a qual:GeometricQualityInformation</rdfs:comment>
        <rdfs:label>reflects geometric quality</rdfs:label>
    </owl:ObjectProperty>
    


    <!-- 
    ///////////////////////////////////////////////////////////////////////////////////////
    //
    // Data properties
    //
    ///////////////////////////////////////////////////////////////////////////////////////
     -->


    


    <!-- http://purl.org/dc/terms/description -->


    <owl:DatatypeProperty rdf:about="http://purl.org/dc/terms/description">
        <rdfs:label>description</rdfs:label>
    </owl:DatatypeProperty>
    


    <!-- http://purl.org/dc/terms/identifier -->


    <owl:DatatypeProperty rdf:about="http://purl.org/dc/terms/identifier">
        <rdfs:label>identifier</rdfs:label>
    </owl:DatatypeProperty>
    


    <!-- http://purl.org/dc/terms/title -->


    <owl:DatatypeProperty rdf:about="http://purl.org/dc/terms/title">
        <rdfs:label>title</rdfs:label>
    </owl:DatatypeProperty>
    


    <!-- https://cogito.iot.linkeddata.es/quality#captureDevice -->


    <owl:DatatypeProperty rdf:about="https://cogito.iot.linkeddata.es/quality#captureDevice">
        <rdfs:comment>Property identifying  the device that has captured an entity (especially a qual:Image)</rdfs:comment>
        <rdfs:label>capture device</rdfs:label>
    </owl:DatatypeProperty>
    


    <!-- https://cogito.iot.linkeddata.es/quality#confidenceLevel -->


    <owl:DatatypeProperty rdf:about="https://cogito.iot.linkeddata.es/quality#confidenceLevel">
        <rdfs:comment>Property indicating the level of confidence of a result (especially a qual:Defect)</rdfs:comment>
        <rdfs:label>confidence level</rdfs:label>
    </owl:DatatypeProperty>
    


    <!-- https://cogito.iot.linkeddata.es/quality#deviceOrientation -->


    <owl:DatatypeProperty rdf:about="https://cogito.iot.linkeddata.es/quality#deviceOrientation">
        <rdfs:comment>Property indicating the orientation of a device</rdfs:comment>
        <rdfs:label>device orientation</rdfs:label>
    </owl:DatatypeProperty>
    


    <!-- https://cogito.iot.linkeddata.es/quality#devicePosition -->


    <owl:DatatypeProperty rdf:about="https://cogito.iot.linkeddata.es/quality#devicePosition">
        <rdfs:comment>Property indication the position of a device</rdfs:comment>
        <rdfs:label>device position</rdfs:label>
    </owl:DatatypeProperty>
    


    <!-- https://cogito.iot.linkeddata.es/quality#elementTypeKeyword -->


    <owl:DatatypeProperty rdf:about="https://cogito.iot.linkeddata.es/quality#elementTypeKeyword">
        <rdfs:comment>List of keywords related to the element type</rdfs:comment>
        <rdfs:label>element type keywords</rdfs:label>
    </owl:DatatypeProperty>
    


    <!-- https://cogito.iot.linkeddata.es/quality#materialTypeKeyword -->


    <owl:DatatypeProperty rdf:about="https://cogito.iot.linkeddata.es/quality#materialTypeKeyword">
        <rdfs:comment>List of keywords related to the material type</rdfs:comment>
        <rdfs:label>material type keywords</rdfs:label>
    </owl:DatatypeProperty>
    


    <!-- https://cogito.iot.linkeddata.es/quality#originDocument -->


    <owl:DatatypeProperty rdf:about="https://cogito.iot.linkeddata.es/quality#originDocument">
        <rdfs:comment>Property indicating the origin document of an entity (especially a qual:GeometricQualityInformation)</rdfs:comment>
        <rdfs:label>origin document</rdfs:label>
    </owl:DatatypeProperty>
    


    <!-- https://cogito.iot.linkeddata.es/quality#performedTimestamp -->


    <owl:DatatypeProperty rdf:about="https://cogito.iot.linkeddata.es/quality#performedTimestamp">
        <rdfs:comment>Property indicating the actual time</rdfs:comment>
        <rdfs:label>performed timestamp</rdfs:label>
    </owl:DatatypeProperty>
    


    <!-- https://cogito.iot.linkeddata.es/quality#predictedLabel -->


    <owl:DatatypeProperty rdf:about="https://cogito.iot.linkeddata.es/quality#predictedLabel">
        <rdfs:comment>Property indicating the origin document of an entity (especially a qual:Defect)</rdfs:comment>
        <rdfs:label>predicted label</rdfs:label>
    </owl:DatatypeProperty>
    


    <!-- https://cogito.iot.linkeddata.es/quality#relationshipTypeKeyword -->


    <owl:DatatypeProperty rdf:about="https://cogito.iot.linkeddata.es/quality#relationshipTypeKeyword">
        <rdfs:comment>List of keywords related to the relationship type</rdfs:comment>
        <rdfs:label>relationship type keywords</rdfs:label>
    </owl:DatatypeProperty>
    


    <!-- https://cogito.iot.linkeddata.es/quality#result -->


    <owl:DatatypeProperty rdf:about="https://cogito.iot.linkeddata.es/quality#result">
        <rdfs:comment>Property indicating the result of an entity (especially a qual:GeometricQualityInformation</rdfs:comment>
        <rdfs:label>result</rdfs:label>
    </owl:DatatypeProperty>
    


    <!-- https://cogito.iot.linkeddata.es/quality#scalarResult -->


    <owl:DatatypeProperty rdf:about="https://cogito.iot.linkeddata.es/quality#scalarResult">
        <rdfs:comment>Property indicating the scalar result</rdfs:comment>
        <rdfs:label>scalar result</rdfs:label>
    </owl:DatatypeProperty>
    


    <!-- https://cogito.iot.linkeddata.es/quality#scheduledTimestamp -->


    <owl:DatatypeProperty rdf:about="https://cogito.iot.linkeddata.es/quality#scheduledTimestamp">
        <rdfs:comment>Property indicating the scheduled time</rdfs:comment>
        <rdfs:label>scheduled timestamp</rdfs:label>
    </owl:DatatypeProperty>
    


    <!-- https://cogito.iot.linkeddata.es/quality#severity -->


    <owl:DatatypeProperty rdf:about="https://cogito.iot.linkeddata.es/quality#severity">
        <rdfs:comment>A property indicating the severity of an entity (especially a qual:Defect)</rdfs:comment>
        <rdfs:label>severity</rdfs:label>
    </owl:DatatypeProperty>
    


    <!-- https://cogito.iot.linkeddata.es/quality#status -->


    <owl:DatatypeProperty rdf:about="https://cogito.iot.linkeddata.es/quality#status">
        <rdfs:comment>Property indicating if a result has been reviewed, confirmed or rejected</rdfs:comment>
        <rdfs:label>status</rdfs:label>
    </owl:DatatypeProperty>
    


    <!-- https://cogito.iot.linkeddata.es/quality#takenAtTime -->


    <owl:DatatypeProperty rdf:about="https://cogito.iot.linkeddata.es/quality#takenAtTime">
        <rdfs:comment>Property indicating the time a data has been taken</rdfs:comment>
        <rdfs:label>taken at time</rdfs:label>
    </owl:DatatypeProperty>
    


    <!-- https://cogito.iot.linkeddata.es/quality#toleranceReference -->


    <owl:DatatypeProperty rdf:about="https://cogito.iot.linkeddata.es/quality#toleranceReference">
        <rdfs:comment>property indicating the tolerance reference</rdfs:comment>
        <rdfs:label>tolerance reference</rdfs:label>
    </owl:DatatypeProperty>
    


    <!-- https://cogito.iot.linkeddata.es/quality#unit -->


    <owl:DatatypeProperty rdf:about="https://cogito.iot.linkeddata.es/quality#unit">
        <rdfs:comment>Property indicating the unit of an entity</rdfs:comment>
        <rdfs:label>unit</rdfs:label>
    </owl:DatatypeProperty>
    


    <!-- 
    ///////////////////////////////////////////////////////////////////////////////////////
    //
    // Classes
    //
    ///////////////////////////////////////////////////////////////////////////////////////
     -->


    


    <!-- https://cogito.iot.linkeddata.es/def/facility#Element -->


    <owl:Class rdf:about="https://cogito.iot.linkeddata.es/def/facility#Element">
        <rdfs:comment>A subclass or bot:Element and, as such, a constituent of a construction entity with a characteristic technical function, form, or position</rdfs:comment>
        <rdfs:label>Element</rdfs:label>
    </owl:Class>
    


    <!-- https://cogito.iot.linkeddata.es/def/facility#Project -->


    <owl:Class rdf:about="https://cogito.iot.linkeddata.es/def/facility#Project">
        <rdfs:comment>A large or major undertaking, especially one involving considerable money, personnel, and equipment</rdfs:comment>
        <rdfs:label>Project</rdfs:label>
    </owl:Class>
    


    <!-- https://cogito.iot.linkeddata.es/process#WorkOrder -->


    <owl:Class rdf:about="https://cogito.iot.linkeddata.es/process#WorkOrder">
        <rdfs:comment>A command or instruction authorizing specific work, repairs, etc., to be done</rdfs:comment>
        <rdfs:label>Work Order</rdfs:label>
    </owl:Class>
    


    <!-- https://cogito.iot.linkeddata.es/quality#AsBuiltMesh -->


    <owl:Class rdf:about="https://cogito.iot.linkeddata.es/quality#AsBuiltMesh">
        <rdfs:subClassOf rdf:resource="https://cogito.iot.linkeddata.es/quality#Mesh"/>
        <rdfs:comment>A mesh representing a built entity (especially a facility:Element)</rdfs:comment>
        <rdfs:label>As-built Mesh</rdfs:label>
    </owl:Class>
    


    <!-- https://cogito.iot.linkeddata.es/quality#AsBuiltPointCloud -->


    <owl:Class rdf:about="https://cogito.iot.linkeddata.es/quality#AsBuiltPointCloud">
        <rdfs:subClassOf rdf:resource="https://cogito.iot.linkeddata.es/quality#PointCoud"/>
        <rdfs:comment>A point cloud representing a built entity (especially a facility:Element)</rdfs:comment>
        <rdfs:label>As-built Point Cloud</rdfs:label>
    </owl:Class>
    


    <!-- https://cogito.iot.linkeddata.es/quality#Defect -->


    <owl:Class rdf:about="https://cogito.iot.linkeddata.es/quality#Defect">
        <rdfs:subClassOf rdf:resource="https://cogito.iot.linkeddata.es/quality#QualityResult"/>
        <rdfs:comment>A shortcoming, fault, or imperfection regarding a particular facility:Element.</rdfs:comment>
        <rdfs:label>Defect</rdfs:label>
    </owl:Class>
    


    <!-- https://cogito.iot.linkeddata.es/quality#GeometricQualityInformation -->


    <owl:Class rdf:about="https://cogito.iot.linkeddata.es/quality#GeometricQualityInformation">
        <rdfs:subClassOf rdf:resource="https://cogito.iot.linkeddata.es/quality#QualityResult"/>
        <rdfs:comment>Data informing a particular problem regarding a particular qual:Rule on a facility:Element</rdfs:comment>
        <rdfs:label>Geometric Quality Information</rdfs:label>
    </owl:Class>
    


    <!-- https://cogito.iot.linkeddata.es/quality#Image -->


    <owl:Class rdf:about="https://cogito.iot.linkeddata.es/quality#Image">
        <rdfs:subClassOf rdf:resource="https://cogito.iot.linkeddata.es/quality#InformationResource"/>
        <rdfs:comment>A picture of an entity</rdfs:comment>
        <rdfs:label>Image</rdfs:label>
    </owl:Class>
    


    <!-- https://cogito.iot.linkeddata.es/quality#ImageJob -->


    <owl:Class rdf:about="https://cogito.iot.linkeddata.es/quality#ImageJob">
        <rdfs:subClassOf rdf:resource="https://cogito.iot.linkeddata.es/quality#InformationResource"/>
        <rdfs:comment>Data regarding an image and the results of processing it</rdfs:comment>
        <rdfs:label>Image Job</rdfs:label>
    </owl:Class>
    


    <!-- https://cogito.iot.linkeddata.es/quality#InformationResource -->


    <owl:Class rdf:about="https://cogito.iot.linkeddata.es/quality#InformationResource">
        <rdfs:comment>Data regarding  the quality of an entity (especially a facility:Project or facility:Element) and that may have associated files</rdfs:comment>
        <rdfs:label>Quality Information</rdfs:label>
    </owl:Class>
    


    <!-- https://cogito.iot.linkeddata.es/quality#Mesh -->


    <owl:Class rdf:about="https://cogito.iot.linkeddata.es/quality#Mesh">
        <rdfs:subClassOf rdf:resource="https://cogito.iot.linkeddata.es/quality#InformationResource"/>
        <rdfs:comment>A collection of vertices, edges and faces that defines the shape of an object (especially a facility:Element)</rdfs:comment>
        <rdfs:label>Mesh</rdfs:label>
    </owl:Class>
    


    <!-- https://cogito.iot.linkeddata.es/quality#PointCoud -->


    <owl:Class rdf:about="https://cogito.iot.linkeddata.es/quality#PointCoud">
        <rdfs:subClassOf rdf:resource="https://cogito.iot.linkeddata.es/quality#InformationResource"/>
        <rdfs:comment>A set of data points in space</rdfs:comment>
        <rdfs:label>Point Cloud</rdfs:label>
    </owl:Class>
    


    <!-- https://cogito.iot.linkeddata.es/quality#QualityResult -->


    <owl:Class rdf:about="https://cogito.iot.linkeddata.es/quality#QualityResult">
        <rdfs:comment>The result of the analysis of  information (especially qual:QuantityInformation)</rdfs:comment>
        <rdfs:label>Quality Result</rdfs:label>
    </owl:Class>
    


    <!-- https://cogito.iot.linkeddata.es/quality#RawImage -->


    <owl:Class rdf:about="https://cogito.iot.linkeddata.es/quality#RawImage">
        <rdfs:subClassOf rdf:resource="https://cogito.iot.linkeddata.es/quality#Image"/>
        <rdfs:comment>An image that has not been processed</rdfs:comment>
        <rdfs:label>Raw Image</rdfs:label>
    </owl:Class>
    


    <!-- https://cogito.iot.linkeddata.es/quality#Rule -->


    <owl:Class rdf:about="https://cogito.iot.linkeddata.es/quality#Rule">
        <rdfs:comment>Information regarding what an entity (especially a faciity:Element) must fulfil</rdfs:comment>
        <rdfs:label>Rule</rdfs:label>
    </owl:Class>
</rdf:RDF>



<!-- Generated by the OWL API (version 5.1.14) https://github.com/owlcs/owlapi/ -->


