@prefix : <https://cogito.iot.linkeddata.es/quality#> .
@prefix owl: <http://www.w3.org/2002/07/owl#> .
@prefix rdf: <http://www.w3.org/1999/02/22-rdf-syntax-ns#> .
@prefix xml: <http://www.w3.org/XML/1998/namespace> .
@prefix xsd: <http://www.w3.org/2001/XMLSchema#> .
@prefix rdfs: <http://www.w3.org/2000/01/rdf-schema#> .
@base <https://cogito.iot.linkeddata.es/quality#> .

<https://cogito.iot.linkeddata.es/quality#> rdf:type owl:Ontology ;
                                             <http://purl.org/dc/elements/1.1/creator> "María Poveda Villalón" ,
                                                                                       "Raúl García Castro" ,
                                                                                       "Socorro  Bernardos Galindo" ;
                                             <http://purl.org/dc/elements/1.1/description> "The COGITO Quality ontology aims at modelling the construction quality domain." ;
                                             <http://purl.org/dc/elements/1.1/title> "Quality Ontology" ;
                                             <http://purl.org/dc/terms/license> <http://purl.org/NET/rdflicense/cc-by4.0> ;
                                             owl:versionInfo "0.9.0" .

#################################################################
#    Annotation properties
#################################################################

###  http://purl.org/dc/elements/1.1/creator
<http://purl.org/dc/elements/1.1/creator> rdf:type owl:AnnotationProperty .


###  http://purl.org/dc/elements/1.1/description
<http://purl.org/dc/elements/1.1/description> rdf:type owl:AnnotationProperty .


###  http://purl.org/dc/elements/1.1/title
<http://purl.org/dc/elements/1.1/title> rdf:type owl:AnnotationProperty .


###  http://purl.org/dc/terms/license
<http://purl.org/dc/terms/license> rdf:type owl:AnnotationProperty .


#################################################################
#    Object Properties
#################################################################

###  https://cogito.iot.linkeddata.es/def/quality#isRelatedToProject
<https://cogito.iot.linkeddata.es/def/quality#isRelatedToProject> rdf:type owl:ObjectProperty ;
                                                                  rdfs:range <https://cogito.iot.linkeddata.es/def/facility#Project> ;
                                                                  rdfs:comment "Property that relates an entity (especially qual:QualityInformation and quel:Rule) to a facility:Project" ;
                                                                  rdfs:label "is related to project" .


###  https://cogito.iot.linkeddata.es/quality#hasProcessedImage
:hasProcessedImage rdf:type owl:ObjectProperty ;
                   rdfs:range :Image ;
                   rdfs:comment "Property that relates an entity (especially qual:ImageJob to a processed qual:Image" ;
                   rdfs:label "has processed image" .


###  https://cogito.iot.linkeddata.es/quality#hasRawImage
:hasRawImage rdf:type owl:ObjectProperty ;
             rdfs:subPropertyOf owl:topObjectProperty ;
             rdfs:range :RawImage ;
             rdfs:comment "Property that relates an entity (especially qual:ImageJob to an original qual:Image" ;
             rdfs:label "has raw image" .


###  https://cogito.iot.linkeddata.es/quality#hasResultImage
:hasResultImage rdf:type owl:ObjectProperty ;
                rdfs:range :Image ;
                rdfs:comment "Property that relates an entity (especially qual:ImageJob to a resulting qual:Image" ;
                rdfs:label "has result image" .


###  https://cogito.iot.linkeddata.es/quality#isRelatedToElement
:isRelatedToElement rdf:type owl:ObjectProperty ;
                    rdfs:range <https://cogito.iot.linkeddata.es/def/facility#Element> ;
                    rdfs:comment "Property that relates an entity (especially qual:QualityInformation) to a facility:Element" ;
                    rdfs:label "is related to element" .


###  https://cogito.iot.linkeddata.es/quality#isRelatedToWorkOrder
:isRelatedToWorkOrder rdf:type owl:ObjectProperty ;
                      rdfs:range <https://cogito.iot.linkeddata.es/process#WorkOrder> ;
                      rdfs:comment "Property that relates an entity (especially qual:QuqlityInformation) to a process:WorkOrder" ;
                      rdfs:label "is related to work order" .


###  https://cogito.iot.linkeddata.es/quality#refelctsQualityResult
:refelctsQualityResult rdf:type owl:ObjectProperty ;
                       rdfs:comment "Property that relates an entity (especially qual:QuqlityInformation to a qual:QualityResult" ;
                       rdfs:label "reflects quality result" .


###  https://cogito.iot.linkeddata.es/quality#refersToElement
:refersToElement rdf:type owl:ObjectProperty ;
                 rdfs:range <https://cogito.iot.linkeddata.es/def/facility#Element> ;
                 rdfs:comment "Property that relates an entity (especially qual:QualityResult) to a facility:Element" ;
                 rdfs:label "refers to element" .


###  https://cogito.iot.linkeddata.es/quality#refersToRule
:refersToRule rdf:type owl:ObjectProperty ;
              rdfs:range :Rule ;
              rdfs:comment "Property that relates an entity (especially qual:Defect) to a qual:Rule" ;
              rdfs:label "refers to rule" .


###  https://cogito.iot.linkeddata.es/quality#reflectsDefect
:reflectsDefect rdf:type owl:ObjectProperty ;
                rdfs:subPropertyOf :refelctsQualityResult ;
                rdfs:range :Defect ;
                rdfs:comment "Property that relates an entity (especially qual:ImageJob) to a qual:Defect" ;
                rdfs:label "reflects defect" .


###  https://cogito.iot.linkeddata.es/quality#reflectsGeometricQuality
:reflectsGeometricQuality rdf:type owl:ObjectProperty ;
                          rdfs:subPropertyOf :refelctsQualityResult ;
                          rdfs:range :GeometricQualityInformation ;
                          rdfs:comment "Property that relates an entity (especially qual:PointCloud) to a qual:GeometricQualityInformation" ;
                          rdfs:label "reflects geometric quality" .


#################################################################
#    Data properties
#################################################################

###  http://purl.org/dc/terms/description
<http://purl.org/dc/terms/description> rdf:type owl:DatatypeProperty ;
                                       rdfs:label "description" .


###  http://purl.org/dc/terms/identifier
<http://purl.org/dc/terms/identifier> rdf:type owl:DatatypeProperty ;
                                      rdfs:label "identifier" .


###  http://purl.org/dc/terms/title
<http://purl.org/dc/terms/title> rdf:type owl:DatatypeProperty ;
                                 rdfs:label "title" .


###  https://cogito.iot.linkeddata.es/quality#captureDevice
:captureDevice rdf:type owl:DatatypeProperty ;
               rdfs:comment "Property identifying  the device that has captured an entity (especially a qual:Image)" ;
               rdfs:label "capture device" .


###  https://cogito.iot.linkeddata.es/quality#confidenceLevel
:confidenceLevel rdf:type owl:DatatypeProperty ;
                 rdfs:comment "Property indicating the level of confidence of a result (especially a qual:Defect)" ;
                 rdfs:label "confidence level" .


###  https://cogito.iot.linkeddata.es/quality#deviceOrientation
:deviceOrientation rdf:type owl:DatatypeProperty ;
                   rdfs:comment "Property indicating the orientation of a device" ;
                   rdfs:label "device orientation" .


###  https://cogito.iot.linkeddata.es/quality#devicePosition
:devicePosition rdf:type owl:DatatypeProperty ;
                rdfs:comment "Property indication the position of a device" ;
                rdfs:label "device position" .


###  https://cogito.iot.linkeddata.es/quality#elementTypeKeyword
:elementTypeKeyword rdf:type owl:DatatypeProperty ;
                    rdfs:comment "List of keywords related to the element type" ;
                    rdfs:label "element type keywords" .


###  https://cogito.iot.linkeddata.es/quality#materialTypeKeyword
:materialTypeKeyword rdf:type owl:DatatypeProperty ;
                     rdfs:comment "List of keywords related to the material type" ;
                     rdfs:label "material type keywords" .


###  https://cogito.iot.linkeddata.es/quality#originDocument
:originDocument rdf:type owl:DatatypeProperty ;
                rdfs:comment "Property indicating the origin document of an entity (especially a qual:GeometricQualityInformation)" ;
                rdfs:label "origin document" .


###  https://cogito.iot.linkeddata.es/quality#performedTimestamp
:performedTimestamp rdf:type owl:DatatypeProperty ;
                    rdfs:comment "Property indicating the actual time" ;
                    rdfs:label "performed timestamp" .


###  https://cogito.iot.linkeddata.es/quality#predictedLabel
:predictedLabel rdf:type owl:DatatypeProperty ;
                rdfs:comment "Property indicating the origin document of an entity (especially a qual:Defect)" ;
                rdfs:label "predicted label" .


###  https://cogito.iot.linkeddata.es/quality#relationshipTypeKeyword
:relationshipTypeKeyword rdf:type owl:DatatypeProperty ;
                         rdfs:comment "List of keywords related to the relationship type" ;
                         rdfs:label "relationship type keywords" .


###  https://cogito.iot.linkeddata.es/quality#result
:result rdf:type owl:DatatypeProperty ;
        rdfs:comment "Property indicating the result of an entity (especially a qual:GeometricQualityInformation" ;
        rdfs:label "result" .


###  https://cogito.iot.linkeddata.es/quality#scalarResult
:scalarResult rdf:type owl:DatatypeProperty ;
              rdfs:comment "Property indicating the scalar result" ;
              rdfs:label "scalar result" .


###  https://cogito.iot.linkeddata.es/quality#scheduledTimestamp
:scheduledTimestamp rdf:type owl:DatatypeProperty ;
                    rdfs:comment "Property indicating the scheduled time" ;
                    rdfs:label "scheduled timestamp" .


###  https://cogito.iot.linkeddata.es/quality#severity
:severity rdf:type owl:DatatypeProperty ;
          rdfs:comment "A property indicating the severity of an entity (especially a qual:Defect)" ;
          rdfs:label "severity" .


###  https://cogito.iot.linkeddata.es/quality#status
:status rdf:type owl:DatatypeProperty ;
        rdfs:comment "Property indicating if a result has been reviewed, confirmed or rejected" ;
        rdfs:label "status" .


###  https://cogito.iot.linkeddata.es/quality#takenAtTime
:takenAtTime rdf:type owl:DatatypeProperty ;
             rdfs:comment "Property indicating the time a data has been taken" ;
             rdfs:label "taken at time" .


###  https://cogito.iot.linkeddata.es/quality#toleranceReference
:toleranceReference rdf:type owl:DatatypeProperty ;
                    rdfs:comment "property indicating the tolerance reference" ;
                    rdfs:label "tolerance reference" .


###  https://cogito.iot.linkeddata.es/quality#unit
:unit rdf:type owl:DatatypeProperty ;
      rdfs:comment "Property indicating the unit of an entity" ;
      rdfs:label "unit" .


#################################################################
#    Classes
#################################################################

###  https://cogito.iot.linkeddata.es/def/facility#Element
<https://cogito.iot.linkeddata.es/def/facility#Element> rdf:type owl:Class ;
                                                        rdfs:comment "A subclass or bot:Element and, as such, a constituent of a construction entity with a characteristic technical function, form, or position" ;
                                                        rdfs:label "Element" .


###  https://cogito.iot.linkeddata.es/def/facility#Project
<https://cogito.iot.linkeddata.es/def/facility#Project> rdf:type owl:Class ;
                                                        rdfs:comment "A large or major undertaking, especially one involving considerable money, personnel, and equipment" ;
                                                        rdfs:label "Project" .


###  https://cogito.iot.linkeddata.es/process#WorkOrder
<https://cogito.iot.linkeddata.es/process#WorkOrder> rdf:type owl:Class ;
                                                     rdfs:comment "A command or instruction authorizing specific work, repairs, etc., to be done" ;
                                                     rdfs:label "Work Order" .


###  https://cogito.iot.linkeddata.es/quality#AsBuiltMesh
:AsBuiltMesh rdf:type owl:Class ;
             rdfs:subClassOf :Mesh ;
             rdfs:comment "A mesh representing a built entity (especially a facility:Element)" ;
             rdfs:label "As-built Mesh" .


###  https://cogito.iot.linkeddata.es/quality#AsBuiltPointCloud
:AsBuiltPointCloud rdf:type owl:Class ;
                   rdfs:subClassOf :PointCoud ;
                   rdfs:comment "A point cloud representing a built entity (especially a facility:Element)" ;
                   rdfs:label "As-built Point Cloud" .


###  https://cogito.iot.linkeddata.es/quality#Defect
:Defect rdf:type owl:Class ;
        rdfs:subClassOf :QualityResult ;
        rdfs:comment "A shortcoming, fault, or imperfection regarding a particular facility:Element." ;
        rdfs:label "Defect" .


###  https://cogito.iot.linkeddata.es/quality#GeometricQualityInformation
:GeometricQualityInformation rdf:type owl:Class ;
                             rdfs:subClassOf :QualityResult ;
                             rdfs:comment "Data informing a particular problem regarding a particular qual:Rule on a facility:Element" ;
                             rdfs:label "Geometric Quality Information" .


###  https://cogito.iot.linkeddata.es/quality#Image
:Image rdf:type owl:Class ;
       rdfs:subClassOf :InformationResource ;
       rdfs:comment "A picture of an entity" ;
       rdfs:label "Image" .


###  https://cogito.iot.linkeddata.es/quality#ImageJob
:ImageJob rdf:type owl:Class ;
          rdfs:subClassOf :InformationResource ;
          rdfs:comment "Data regarding an image and the results of processing it" ;
          rdfs:label "Image Job" .


###  https://cogito.iot.linkeddata.es/quality#InformationResource
:InformationResource rdf:type owl:Class ;
                     rdfs:comment "Data regarding  the quality of an entity (especially a facility:Project or facility:Element) and that may have associated files" ;
                     rdfs:label "Quality Information" .


###  https://cogito.iot.linkeddata.es/quality#Mesh
:Mesh rdf:type owl:Class ;
      rdfs:subClassOf :InformationResource ;
      rdfs:comment "A collection of vertices, edges and faces that defines the shape of an object (especially a facility:Element)" ;
      rdfs:label "Mesh" .


###  https://cogito.iot.linkeddata.es/quality#PointCoud
:PointCoud rdf:type owl:Class ;
           rdfs:subClassOf :InformationResource ;
           rdfs:comment "A set of data points in space" ;
           rdfs:label "Point Cloud" .


###  https://cogito.iot.linkeddata.es/quality#QualityResult
:QualityResult rdf:type owl:Class ;
               rdfs:comment "The result of the analysis of  information (especially qual:QuantityInformation)" ;
               rdfs:label "Quality Result" .


###  https://cogito.iot.linkeddata.es/quality#RawImage
:RawImage rdf:type owl:Class ;
          rdfs:subClassOf :Image ;
          rdfs:comment "An image that has not been processed" ;
          rdfs:label "Raw Image" .


###  https://cogito.iot.linkeddata.es/quality#Rule
:Rule rdf:type owl:Class ;
      rdfs:comment "Information regarding what an entity (especially a faciity:Element) must fulfil" ;
      rdfs:label "Rule" .


###  Generated by the OWL API (version 5.1.14) https://github.com/owlcs/owlapi/
