<?xml version="1.0"?>
<rdf:RDF xmlns="https://cogito.iot.linkeddata.es/def/process#"
     xml:base="https://cogito.iot.linkeddata.es/def/process"
     xmlns:dc="http://purl.org/dc/elements/1.1/"
     xmlns:owl="http://www.w3.org/2002/07/owl#"
     xmlns:rdf="http://www.w3.org/1999/02/22-rdf-syntax-ns#"
     xmlns:xml="http://www.w3.org/XML/1998/namespace"
     xmlns:xsd="http://www.w3.org/2001/XMLSchema#"
     xmlns:rdfs="http://www.w3.org/2000/01/rdf-schema#"
     xmlns:terms="http://purl.org/dc/terms/">
    <owl:Ontology rdf:about="https://cogito.iot.linkeddata.es/def/process#">
        <dc:creator>María Poveda Villalón</dc:creator>
        <dc:creator>Raúl García Castro</dc:creator>
        <dc:creator>Socorro  Bernardos Galindo</dc:creator>
        <dc:description>The COGITO Process ontology aims at modelling the construction process.</dc:description>
        <dc:title>Process Ontology</dc:title>
        <terms:license rdf:resource="http://purl.org/NET/rdflicense/cc-by4.0"/>
        <owl:versionInfo>0.11.0</owl:versionInfo>
    </owl:Ontology>
    


    <!-- 
    ///////////////////////////////////////////////////////////////////////////////////////
    //
    // Annotation properties
    //
    ///////////////////////////////////////////////////////////////////////////////////////
     -->


    


    <!-- http://purl.org/dc/elements/1.1/creator -->


    <owl:AnnotationProperty rdf:about="http://purl.org/dc/elements/1.1/creator"/>
    


    <!-- http://purl.org/dc/elements/1.1/description -->


    <owl:AnnotationProperty rdf:about="http://purl.org/dc/elements/1.1/description"/>
    


    <!-- http://purl.org/dc/elements/1.1/title -->


    <owl:AnnotationProperty rdf:about="http://purl.org/dc/elements/1.1/title"/>
    


    <!-- http://purl.org/dc/terms/license -->


    <owl:AnnotationProperty rdf:about="http://purl.org/dc/terms/license"/>
    


    <!-- 
    ///////////////////////////////////////////////////////////////////////////////////////
    //
    // Object Properties
    //
    ///////////////////////////////////////////////////////////////////////////////////////
     -->


    


    <!-- https://cogito.iot.linkeddata.es/def/process#addsElement -->


    <owl:ObjectProperty rdf:about="https://cogito.iot.linkeddata.es/def/process#addsElement">
        <owl:inverseOf rdf:resource="https://cogito.iot.linkeddata.es/def/process#isAddedByTask"/>
        <rdfs:comment>A property that relates an entity (especially a process:Task) to the facility:Element it creates</rdfs:comment>
        <rdfs:label>adds element</rdfs:label>
    </owl:ObjectProperty>
    


    <!-- https://cogito.iot.linkeddata.es/def/process#belongsToProcess -->


    <owl:ObjectProperty rdf:about="https://cogito.iot.linkeddata.es/def/process#belongsToProcess">
        <owl:inverseOf rdf:resource="https://cogito.iot.linkeddata.es/def/process#hasTask"/>
        <rdfs:range rdf:resource="https://cogito.iot.linkeddata.es/def/process#Process"/>
        <rdfs:comment>A property that relates an entity (especially a process:Task) to the process:Process it belongs to</rdfs:comment>
        <rdfs:label>belongs to process</rdfs:label>
    </owl:ObjectProperty>
    


    <!-- https://cogito.iot.linkeddata.es/def/process#controlsElement -->


    <owl:ObjectProperty rdf:about="https://cogito.iot.linkeddata.es/def/process#controlsElement">
        <owl:inverseOf rdf:resource="https://cogito.iot.linkeddata.es/def/process#isControlledByTask"/>
        <rdfs:range rdf:resource="https://cogito.iot.linkeddata.es/def/facility#Element"/>
        <rdfs:comment>A property that relates an entity (especially a process:Task) to the facility:Element it controls</rdfs:comment>
        <rdfs:label>controls element</rdfs:label>
    </owl:ObjectProperty>
    


    <!-- https://cogito.iot.linkeddata.es/def/process#hasComponentTask -->


    <owl:ObjectProperty rdf:about="https://cogito.iot.linkeddata.es/def/process#hasComponentTask">
        <rdfs:range rdf:resource="https://cogito.iot.linkeddata.es/def/process#Task"/>
        <rdfs:comment>A property that relates an entity (especially a process:WorkOrder) to its tasks</rdfs:comment>
        <rdfs:label>has component task</rdfs:label>
    </owl:ObjectProperty>
    


    <!-- https://cogito.iot.linkeddata.es/def/process#hasCost -->


    <owl:ObjectProperty rdf:about="https://cogito.iot.linkeddata.es/def/process#hasCost">
        <rdfs:range rdf:resource="https://cogito.iot.linkeddata.es/def/process#Cost"/>
        <rdfs:comment>A property that relates an entity (especially a process:Task or a process:Process) to its cost</rdfs:comment>
        <rdfs:label>has cost</rdfs:label>
    </owl:ObjectProperty>
    


    <!-- https://cogito.iot.linkeddata.es/def/process#hasMainProvider -->


    <owl:ObjectProperty rdf:about="https://cogito.iot.linkeddata.es/def/process#hasMainProvider">
        <rdfs:range rdf:resource="https://cogito.iot.linkeddata.es/def/resource#Worker"/>
        <rdfs:comment>A property that relates an entity (especially a process:WorkOrder) to the resource:Worker that acts as its main provider</rdfs:comment>
        <rdfs:label>has main provider</rdfs:label>
    </owl:ObjectProperty>
    


    <!-- https://cogito.iot.linkeddata.es/def/process#hasResourceTypeRequirement -->


    <owl:ObjectProperty rdf:about="https://cogito.iot.linkeddata.es/def/process#hasResourceTypeRequirement">
        <rdfs:range rdf:resource="https://cogito.iot.linkeddata.es/def/process#ResourceTypeRequirement"/>
        <rdfs:comment>Aproperty that relates an entity (especially a process:Task) to its requirements of resource types:</rdfs:comment>
        <rdfs:label>has resource type requirement</rdfs:label>
    </owl:ObjectProperty>
    


    <!-- https://cogito.iot.linkeddata.es/def/process#hasSubTask -->


    <owl:ObjectProperty rdf:about="https://cogito.iot.linkeddata.es/def/process#hasSubTask">
        <owl:inverseOf rdf:resource="https://cogito.iot.linkeddata.es/def/process#isSubTaskOf"/>
        <rdfs:range rdf:resource="https://cogito.iot.linkeddata.es/def/process#Task"/>
        <rdfs:comment>A property that relates an entity (especially a process:Task) to the tasks it includes</rdfs:comment>
        <rdfs:label>has sub-task</rdfs:label>
    </owl:ObjectProperty>
    


    <!-- https://cogito.iot.linkeddata.es/def/process#hasTask -->


    <owl:ObjectProperty rdf:about="https://cogito.iot.linkeddata.es/def/process#hasTask">
        <rdfs:range rdf:resource="https://cogito.iot.linkeddata.es/def/process#Task"/>
        <rdfs:comment>A property that relates an entity (especially a process:Process) to the tasks it involves</rdfs:comment>
        <rdfs:label>has task</rdfs:label>
    </owl:ObjectProperty>
    


    <!-- https://cogito.iot.linkeddata.es/def/process#hasWorkOrder -->


    <owl:ObjectProperty rdf:about="https://cogito.iot.linkeddata.es/def/process#hasWorkOrder">
        <rdfs:range rdf:resource="https://cogito.iot.linkeddata.es/def/process#WorkOrder"/>
        <rdfs:comment>A property that relates an entity (especially a process:Process) to the work orders it contains</rdfs:comment>
        <rdfs:label>has work order</rdfs:label>
    </owl:ObjectProperty>
    


    <!-- https://cogito.iot.linkeddata.es/def/process#involvesResourceType -->


    <owl:ObjectProperty rdf:about="https://cogito.iot.linkeddata.es/def/process#involvesResourceType">
        <rdfs:range rdf:resource="https://cogito.iot.linkeddata.es/def/resource#ResourceType"/>
        <rdfs:comment>A property that relates an entity (especially a process:Process) to the resource types it includes</rdfs:comment>
        <rdfs:label>involves resource type</rdfs:label>
    </owl:ObjectProperty>
    


    <!-- https://cogito.iot.linkeddata.es/def/process#isAddedByTask -->


    <owl:ObjectProperty rdf:about="https://cogito.iot.linkeddata.es/def/process#isAddedByTask">
        <rdfs:range rdf:resource="https://cogito.iot.linkeddata.es/def/process#Task"/>
        <rdfs:comment>A property that relates an entity (especially a  facility:Element) to the process:Task  that creates it</rdfs:comment>
        <rdfs:label>is added by task</rdfs:label>
    </owl:ObjectProperty>
    


    <!-- https://cogito.iot.linkeddata.es/def/process#isControlledByTask -->


    <owl:ObjectProperty rdf:about="https://cogito.iot.linkeddata.es/def/process#isControlledByTask">
        <rdfs:range rdf:resource="https://cogito.iot.linkeddata.es/def/process#Task"/>
        <rdfs:comment>A property that relates an entity (especially a  facility:Element)  to the process:Task  that controls it</rdfs:comment>
        <rdfs:label>is controlled by task</rdfs:label>
    </owl:ObjectProperty>
    


    <!-- https://cogito.iot.linkeddata.es/def/process#isExecutedAfter -->


    <owl:ObjectProperty rdf:about="https://cogito.iot.linkeddata.es/def/process#isExecutedAfter">
        <rdfs:domain rdf:resource="https://cogito.iot.linkeddata.es/def/process#Task"/>
        <rdfs:range rdf:resource="https://cogito.iot.linkeddata.es/def/process#Task"/>
        <rdfs:comment>A property that relates an entity (especially a process:Task) to the task that have to be executed before it</rdfs:comment>
        <rdfs:label>is executed after</rdfs:label>
    </owl:ObjectProperty>
    


    <!-- https://cogito.iot.linkeddata.es/def/process#isMeasuredIn -->


    <owl:ObjectProperty rdf:about="https://cogito.iot.linkeddata.es/def/process#isMeasuredIn">
        <rdfs:range rdf:resource="https://cogito.iot.linkeddata.es/def/process#UnitOfCurrency"/>
        <rdfs:comment>A property that relates an entity (especially a process:Cost) to the currency it is measured in</rdfs:comment>
        <rdfs:label>is measured in</rdfs:label>
    </owl:ObjectProperty>
    


    <!-- https://cogito.iot.linkeddata.es/def/process#isRelatedToProcess -->


    <owl:ObjectProperty rdf:about="https://cogito.iot.linkeddata.es/def/process#isRelatedToProcess">
        <owl:inverseOf rdf:resource="https://cogito.iot.linkeddata.es/def/process#isRelatedToProject"/>
        <rdfs:range rdf:resource="https://cogito.iot.linkeddata.es/def/process#Process"/>
        <rdfs:comment>A property that relates an entity (especially a facility:Project) to its processes</rdfs:comment>
        <rdfs:label>is related to process</rdfs:label>
    </owl:ObjectProperty>
    


    <!-- https://cogito.iot.linkeddata.es/def/process#isRelatedToProject -->


    <owl:ObjectProperty rdf:about="https://cogito.iot.linkeddata.es/def/process#isRelatedToProject">
        <rdfs:range rdf:resource="https://cogito.iot.linkeddata.es/def/facility#Project"/>
        <rdfs:comment>A property that relates an entity (especially a process:Process) to its facility:Project</rdfs:comment>
        <rdfs:label>is related to project</rdfs:label>
    </owl:ObjectProperty>
    


    <!-- https://cogito.iot.linkeddata.es/def/process#isRemovedByTask -->


    <owl:ObjectProperty rdf:about="https://cogito.iot.linkeddata.es/def/process#isRemovedByTask">
        <owl:inverseOf rdf:resource="https://cogito.iot.linkeddata.es/def/process#removesElement"/>
        <rdfs:range rdf:resource="https://cogito.iot.linkeddata.es/def/process#Task"/>
        <rdfs:comment>A property that relates an entity (especially a  facility:Element)  to the process:Task  that removes it</rdfs:comment>
        <rdfs:label>is removed by task</rdfs:label>
    </owl:ObjectProperty>
    


    <!-- https://cogito.iot.linkeddata.es/def/process#isRepairedByTask -->


    <owl:ObjectProperty rdf:about="https://cogito.iot.linkeddata.es/def/process#isRepairedByTask">
        <owl:inverseOf rdf:resource="https://cogito.iot.linkeddata.es/def/process#repairsElelment"/>
        <rdfs:range rdf:resource="https://cogito.iot.linkeddata.es/def/process#Task"/>
        <rdfs:comment>A property that relates an entity (especially a  facility:Element)  to the process:Task  that repairs it</rdfs:comment>
        <rdfs:label>is repaired by task</rdfs:label>
    </owl:ObjectProperty>
    


    <!-- https://cogito.iot.linkeddata.es/def/process#isSubTaskOf -->


    <owl:ObjectProperty rdf:about="https://cogito.iot.linkeddata.es/def/process#isSubTaskOf">
        <rdfs:range rdf:resource="https://cogito.iot.linkeddata.es/def/process#Task"/>
        <rdfs:comment>A property that relates an entity (especially a process:Task) to the task it belongs to</rdfs:comment>
        <rdfs:label>is sub-task of</rdfs:label>
    </owl:ObjectProperty>
    


    <!-- https://cogito.iot.linkeddata.es/def/process#relatesToResourceType -->


    <owl:ObjectProperty rdf:about="https://cogito.iot.linkeddata.es/def/process#relatesToResourceType">
        <rdfs:comment>A property that relates an entity (especially a process:ResourceTypeRequirement) to the resource type it refers to</rdfs:comment>
        <rdfs:label>relates to resource type</rdfs:label>
    </owl:ObjectProperty>
    


    <!-- https://cogito.iot.linkeddata.es/def/process#removesElement -->


    <owl:ObjectProperty rdf:about="https://cogito.iot.linkeddata.es/def/process#removesElement">
        <rdfs:range rdf:resource="https://cogito.iot.linkeddata.es/def/facility#Element"/>
        <rdfs:comment>A property that relates a process:Task to the facility:Element it removes</rdfs:comment>
        <rdfs:label>removes element</rdfs:label>
    </owl:ObjectProperty>
    


    <!-- https://cogito.iot.linkeddata.es/def/process#repairsElelment -->


    <owl:ObjectProperty rdf:about="https://cogito.iot.linkeddata.es/def/process#repairsElelment">
        <rdfs:range rdf:resource="https://cogito.iot.linkeddata.es/def/facility#Element"/>
        <rdfs:comment>A property that relates a process:Task to the facility:Element it repairs</rdfs:comment>
        <rdfs:label>repairs element</rdfs:label>
    </owl:ObjectProperty>
    


    <!-- https://cogito.iot.linkeddata.es/def/resource#belongsToResourceType -->


    <owl:ObjectProperty rdf:about="https://cogito.iot.linkeddata.es/def/resource#belongsToResourceType">
        <rdfs:range rdf:resource="https://cogito.iot.linkeddata.es/def/resource#ResourceType"/>
        <rdfs:comment>A property that relates a resource:Resource to its type</rdfs:comment>
        <rdfs:label>belongs to resource type</rdfs:label>
    </owl:ObjectProperty>
    


    <!-- https://cogito.iot.linkeddata.es/def/resource#hasAssignedResource -->


    <owl:ObjectProperty rdf:about="https://cogito.iot.linkeddata.es/def/resource#hasAssignedResource">
        <rdfs:range rdf:resource="https://cogito.iot.linkeddata.es/def/resource#Resource"/>
        <rdfs:comment>A property that relates an entity (especially a process:Task) to the resource:Resource it has assigned</rdfs:comment>
        <rdfs:label>has assigned resource</rdfs:label>
    </owl:ObjectProperty>
    


    <!-- 
    ///////////////////////////////////////////////////////////////////////////////////////
    //
    // Data properties
    //
    ///////////////////////////////////////////////////////////////////////////////////////
     -->


    


    <!-- http://purl.org/dc/terms/created -->


    <owl:DatatypeProperty rdf:about="http://purl.org/dc/terms/created">
        <rdfs:isDefinedBy rdf:resource="http://purl.org/dc/terms/"/>
        <rdfs:label rdf:resource="https://cogito.iot.linkeddata.es/def/created"/>
    </owl:DatatypeProperty>
    


    <!-- http://purl.org/dc/terms/creator -->


    <owl:DatatypeProperty rdf:about="http://purl.org/dc/terms/creator">
        <rdfs:isDefinedBy rdf:resource="http://purl.org/dc/terms/"/>
        <rdfs:label>creator</rdfs:label>
    </owl:DatatypeProperty>
    


    <!-- http://purl.org/dc/terms/description -->


    <owl:DatatypeProperty rdf:about="http://purl.org/dc/terms/description">
        <rdfs:isDefinedBy>http://purl.org/dc/terms</rdfs:isDefinedBy>
        <rdfs:label>description</rdfs:label>
    </owl:DatatypeProperty>
    


    <!-- http://purl.org/dc/terms/identifier -->


    <owl:DatatypeProperty rdf:about="http://purl.org/dc/terms/identifier">
        <rdfs:isDefinedBy rdf:resource="http://purl.org/dc/terms/"/>
        <rdfs:label>identifier</rdfs:label>
    </owl:DatatypeProperty>
    


    <!-- http://purl.org/dc/terms/title -->


    <owl:DatatypeProperty rdf:about="http://purl.org/dc/terms/title">
        <rdfs:isDefinedBy rdf:resource="http://purl.org/dc/terms/"/>
        <rdfs:label>title</rdfs:label>
    </owl:DatatypeProperty>
    


    <!-- https://cogito.iot.linkeddata.es/def/process#actualEndDate -->


    <owl:DatatypeProperty rdf:about="https://cogito.iot.linkeddata.es/def/process#actualEndDate">
        <rdfs:comment>A property indicating the actual end date of an entity</rdfs:comment>
        <rdfs:label>actual end date</rdfs:label>
    </owl:DatatypeProperty>
    


    <!-- https://cogito.iot.linkeddata.es/def/process#actualStartDate -->


    <owl:DatatypeProperty rdf:about="https://cogito.iot.linkeddata.es/def/process#actualStartDate">
        <rdfs:comment>A property indicating the actual start date of an entity</rdfs:comment>
        <rdfs:label>actual start date</rdfs:label>
    </owl:DatatypeProperty>
    


    <!-- https://cogito.iot.linkeddata.es/def/process#amount -->


    <owl:DatatypeProperty rdf:about="https://cogito.iot.linkeddata.es/def/process#amount">
        <rdfs:range rdf:resource="http://www.w3.org/2001/XMLSchema#float"/>
        <rdfs:comment>A property indicating the amount of an entity</rdfs:comment>
        <rdfs:label>amount</rdfs:label>
    </owl:DatatypeProperty>
    


    <!-- https://cogito.iot.linkeddata.es/def/process#crewNumber -->


    <owl:DatatypeProperty rdf:about="https://cogito.iot.linkeddata.es/def/process#crewNumber">
        <rdfs:comment>Property used as resource multiplier factor to specify the number of crews assigned to the task in order to do the work with the provided duration</rdfs:comment>
        <rdfs:label>crew number</rdfs:label>
    </owl:DatatypeProperty>
    


    <!-- https://cogito.iot.linkeddata.es/def/process#crewProductivity -->


    <owl:DatatypeProperty rdf:about="https://cogito.iot.linkeddata.es/def/process#crewProductivity">
        <rdfs:comment>Property indicating  &quot;amount of work / unit of time&quot;. At the moment, we only capture the list of elements to be built, so the productivity values we would use are &quot;units / time&quot;. But, work quantity is typically measured as: m, m2, m3, units, depending on the type of activity. So, we could have a mixture of productivity metrics, m/time, m2/time, m3/time, depending on the type of activity.</rdfs:comment>
        <rdfs:label>crew productivity</rdfs:label>
    </owl:DatatypeProperty>
    


    <!-- https://cogito.iot.linkeddata.es/def/process#crewProductivityPenalty -->


    <owl:DatatypeProperty rdf:about="https://cogito.iot.linkeddata.es/def/process#crewProductivityPenalty">
        <rdfs:comment>Property used as factor to limit the maximum number of crew working in a task</rdfs:comment>
        <rdfs:label>crew productivity penalty</rdfs:label>
    </owl:DatatypeProperty>
    


    <!-- https://cogito.iot.linkeddata.es/def/process#currencyCode -->


    <owl:DatatypeProperty rdf:about="https://cogito.iot.linkeddata.es/def/process#currencyCode">
        <rdfs:comment>A property indicating the currency code of an entity (especially a process:UnitOfCurrency)</rdfs:comment>
        <rdfs:label>currency code</rdfs:label>
    </owl:DatatypeProperty>
    


    <!-- https://cogito.iot.linkeddata.es/def/process#currencySymbol -->


    <owl:DatatypeProperty rdf:about="https://cogito.iot.linkeddata.es/def/process#currencySymbol">
        <rdfs:comment>A property indicating the currency symbol of an entity (especially a process:UnitOfCurrency)</rdfs:comment>
        <rdfs:label>currency symbol</rdfs:label>
    </owl:DatatypeProperty>
    


    <!-- https://cogito.iot.linkeddata.es/def/process#duration -->


    <owl:DatatypeProperty rdf:about="https://cogito.iot.linkeddata.es/def/process#duration">
        <rdfs:range rdf:resource="http://www.w3.org/2001/XMLSchema#nonNegativeInteger"/>
        <rdfs:comment>A property indicating the minimal number of days doing a task takes</rdfs:comment>
        <rdfs:label>duration</rdfs:label>
    </owl:DatatypeProperty>
    


    <!-- https://cogito.iot.linkeddata.es/def/process#isCritical -->


    <owl:DatatypeProperty rdf:about="https://cogito.iot.linkeddata.es/def/process#isCritical">
        <rdfs:range rdf:resource="http://www.w3.org/2001/XMLSchema#boolean"/>
        <rdfs:comment>A property indicating if an entity (especially a task) is critical</rdfs:comment>
        <rdfs:label>is critical</rdfs:label>
    </owl:DatatypeProperty>
    


    <!-- https://cogito.iot.linkeddata.es/def/process#plannedEarlyEndDate -->


    <owl:DatatypeProperty rdf:about="https://cogito.iot.linkeddata.es/def/process#plannedEarlyEndDate">
        <rdfs:range rdf:resource="http://www.w3.org/2001/XMLSchema#dateTimeStamp"/>
        <rdfs:comment>A property indicating the earliest  date an entity can end</rdfs:comment>
        <rdfs:label>planned early end date</rdfs:label>
    </owl:DatatypeProperty>
    


    <!-- https://cogito.iot.linkeddata.es/def/process#plannedEarlyStartDate -->


    <owl:DatatypeProperty rdf:about="https://cogito.iot.linkeddata.es/def/process#plannedEarlyStartDate">
        <rdfs:range rdf:resource="http://www.w3.org/2001/XMLSchema#dateTimeStamp"/>
        <rdfs:comment>A property indicating the earliest  date an entity can start</rdfs:comment>
        <rdfs:label>planned early start date</rdfs:label>
    </owl:DatatypeProperty>
    


    <!-- https://cogito.iot.linkeddata.es/def/process#plannedEndDate -->


    <owl:DatatypeProperty rdf:about="https://cogito.iot.linkeddata.es/def/process#plannedEndDate">
        <rdfs:range rdf:resource="http://www.w3.org/2001/XMLSchema#dateTime"/>
        <rdfs:comment>A property indicating the planned end date of an entity</rdfs:comment>
        <rdfs:label>planned end date</rdfs:label>
    </owl:DatatypeProperty>
    


    <!-- https://cogito.iot.linkeddata.es/def/process#plannedLateEndDate -->


    <owl:DatatypeProperty rdf:about="https://cogito.iot.linkeddata.es/def/process#plannedLateEndDate">
        <rdfs:range rdf:resource="http://www.w3.org/2001/XMLSchema#dateTimeStamp"/>
        <rdfs:comment>A property indicating the latest  date an entity can end</rdfs:comment>
        <rdfs:label>planned late end date</rdfs:label>
    </owl:DatatypeProperty>
    


    <!-- https://cogito.iot.linkeddata.es/def/process#plannedLateStartDate -->


    <owl:DatatypeProperty rdf:about="https://cogito.iot.linkeddata.es/def/process#plannedLateStartDate">
        <rdfs:range rdf:resource="http://www.w3.org/2001/XMLSchema#dateTimeStamp"/>
        <rdfs:comment>A property indicating the latest  date an entity can start</rdfs:comment>
        <rdfs:label>planned late start date</rdfs:label>
    </owl:DatatypeProperty>
    


    <!-- https://cogito.iot.linkeddata.es/def/process#plannedStartDate -->


    <owl:DatatypeProperty rdf:about="https://cogito.iot.linkeddata.es/def/process#plannedStartDate">
        <rdfs:range rdf:resource="http://www.w3.org/2001/XMLSchema#dateTime"/>
        <rdfs:comment>A property indicating the planned start date of an entity</rdfs:comment>
        <rdfs:label>planned start date</rdfs:label>
    </owl:DatatypeProperty>
    


    <!-- https://cogito.iot.linkeddata.es/def/process#priority -->


    <owl:DatatypeProperty rdf:about="https://cogito.iot.linkeddata.es/def/process#priority">
        <rdfs:range rdf:resource="http://www.w3.org/2001/XMLSchema#integer"/>
        <rdfs:comment>A property indicating the priority of an entity</rdfs:comment>
        <rdfs:label>priority</rdfs:label>
    </owl:DatatypeProperty>
    


    <!-- https://cogito.iot.linkeddata.es/def/process#progress -->


    <owl:DatatypeProperty rdf:about="https://cogito.iot.linkeddata.es/def/process#progress">
        <rdfs:range rdf:resource="http://www.w3.org/2001/XMLSchema#float"/>
        <rdfs:comment>A property indicating the progress of an entity (especially a process:Task)</rdfs:comment>
        <rdfs:label>progress</rdfs:label>
    </owl:DatatypeProperty>
    


    <!-- https://cogito.iot.linkeddata.es/def/process#quantityNeeded -->


    <owl:DatatypeProperty rdf:about="https://cogito.iot.linkeddata.es/def/process#quantityNeeded">
        <rdfs:comment>A property indicating the needed quantity of an entity</rdfs:comment>
        <rdfs:label>quantity needed</rdfs:label>
    </owl:DatatypeProperty>
    


    <!-- https://cogito.iot.linkeddata.es/def/process#result -->


    <owl:DatatypeProperty rdf:about="https://cogito.iot.linkeddata.es/def/process#result">
        <rdfs:comment>A property indicating the result of an entity (especially a process:Task)</rdfs:comment>
        <rdfs:label>result</rdfs:label>
    </owl:DatatypeProperty>
    


    <!-- https://cogito.iot.linkeddata.es/def/process#status -->


    <owl:DatatypeProperty rdf:about="https://cogito.iot.linkeddata.es/def/process#status">
        <rdfs:comment>A property indicating the status of an entity (especially a process:WorkOrder)</rdfs:comment>
        <rdfs:label>status</rdfs:label>
    </owl:DatatypeProperty>
    


    <!-- https://cogito.iot.linkeddata.es/def/process#timeStep -->


    <owl:DatatypeProperty rdf:about="https://cogito.iot.linkeddata.es/def/process#timeStep">
        <rdfs:comment>A property indicating the time step of an entity (especially a process:Process)</rdfs:comment>
        <rdfs:label>time step</rdfs:label>
    </owl:DatatypeProperty>
    


    <!-- https://cogito.iot.linkeddata.es/def/process#timeWindow -->


    <owl:DatatypeProperty rdf:about="https://cogito.iot.linkeddata.es/def/process#timeWindow">
        <rdfs:comment>A property indicating the time window of an entity (especially a process:Process)</rdfs:comment>
        <rdfs:label>time window</rdfs:label>
    </owl:DatatypeProperty>
    


    <!-- https://cogito.iot.linkeddata.es/def/process#totalFloat -->


    <owl:DatatypeProperty rdf:about="https://cogito.iot.linkeddata.es/def/process#totalFloat">
        <rdfs:range rdf:resource="http://www.w3.org/2001/XMLSchema#nonNegativeInteger"/>
        <rdfs:comment>A property indicating the number of days an entity (especially a task) can be delayed</rdfs:comment>
        <rdfs:label>total float</rdfs:label>
    </owl:DatatypeProperty>
    


    <!-- https://cogito.iot.linkeddata.es/def/process#workQuantity -->


    <owl:DatatypeProperty rdf:about="https://cogito.iot.linkeddata.es/def/process#workQuantity">
        <rdfs:comment>Property  indicating  the amount of work. Work quantity is typically measured as: m, m2, m3, units, depending on the type of activity. So, we could have a mixture of productivity metrics, m/time, m2/time, m3/time, depending on the type of activity.</rdfs:comment>
        <rdfs:label>work quantity</rdfs:label>
    </owl:DatatypeProperty>
    


    <!-- https://cogito.iot.linkeddata.es/def/process#workQuantityUnit -->


    <owl:DatatypeProperty rdf:about="https://cogito.iot.linkeddata.es/def/process#workQuantityUnit">
        <rdfs:comment>Property indicating the unit used to measure wok quantity. Work quantity is typically measured as: m, m2, m3, units, depending on the type of activity.</rdfs:comment>
        <rdfs:label>work quantity unit</rdfs:label>
    </owl:DatatypeProperty>
    


    <!-- 
    ///////////////////////////////////////////////////////////////////////////////////////
    //
    // Classes
    //
    ///////////////////////////////////////////////////////////////////////////////////////
     -->


    


    <!-- https://cogito.iot.linkeddata.es/def/facility#Element -->


    <owl:Class rdf:about="https://cogito.iot.linkeddata.es/def/facility#Element">
        <rdfs:comment>A subclass or bot:Element and, as such, a constituent of a construction entity with a characteristic technical function, form, or position</rdfs:comment>
        <rdfs:label>Element</rdfs:label>
    </owl:Class>
    


    <!-- https://cogito.iot.linkeddata.es/def/facility#Project -->


    <owl:Class rdf:about="https://cogito.iot.linkeddata.es/def/facility#Project">
        <rdfs:comment>A large or major undertaking, especially one involving considerable money, personnel, and equipment</rdfs:comment>
        <rdfs:label>Project</rdfs:label>
    </owl:Class>
    


    <!-- https://cogito.iot.linkeddata.es/def/process#AsIsProcess -->


    <owl:Class rdf:about="https://cogito.iot.linkeddata.es/def/process#AsIsProcess">
        <rdfs:subClassOf rdf:resource="https://cogito.iot.linkeddata.es/def/process#Process"/>
        <rdfs:comment>A process in its current condition</rdfs:comment>
        <rdfs:label>As-is Process</rdfs:label>
    </owl:Class>
    


    <!-- https://cogito.iot.linkeddata.es/def/process#AsPlannedEnrichedProcess -->


    <owl:Class rdf:about="https://cogito.iot.linkeddata.es/def/process#AsPlannedEnrichedProcess">
        <rdfs:subClassOf rdf:resource="https://cogito.iot.linkeddata.es/def/process#Process"/>
        <rdfs:comment>A planned process after being enriched</rdfs:comment>
        <rdfs:label>As-planned Enriched Process</rdfs:label>
    </owl:Class>
    


    <!-- https://cogito.iot.linkeddata.es/def/process#AsPlannedOriginalProcess -->


    <owl:Class rdf:about="https://cogito.iot.linkeddata.es/def/process#AsPlannedOriginalProcess">
        <rdfs:subClassOf rdf:resource="https://cogito.iot.linkeddata.es/def/process#Process"/>
        <rdfs:comment>An initial planned process</rdfs:comment>
        <rdfs:label>As-planned Original Process</rdfs:label>
    </owl:Class>
    


    <!-- https://cogito.iot.linkeddata.es/def/process#ConstructionTask -->


    <owl:Class rdf:about="https://cogito.iot.linkeddata.es/def/process#ConstructionTask">
        <rdfs:subClassOf rdf:resource="https://cogito.iot.linkeddata.es/def/process#Task"/>
        <rdfs:comment>A task related to a construction domain</rdfs:comment>
        <rdfs:label>Construction Task</rdfs:label>
    </owl:Class>
    


    <!-- https://cogito.iot.linkeddata.es/def/process#Cost -->


    <owl:Class rdf:about="https://cogito.iot.linkeddata.es/def/process#Cost">
        <rdfs:comment>An entity representing the cost of another entity</rdfs:comment>
        <rdfs:label>Cost</rdfs:label>
    </owl:Class>
    


    <!-- https://cogito.iot.linkeddata.es/def/process#GeometricQualityTask -->


    <owl:Class rdf:about="https://cogito.iot.linkeddata.es/def/process#GeometricQualityTask">
        <rdfs:subClassOf rdf:resource="https://cogito.iot.linkeddata.es/def/process#Task"/>
        <rdfs:comment>A task related to the geometric quaity domain</rdfs:comment>
        <rdfs:label>Geometric Quality Task</rdfs:label>
    </owl:Class>
    


    <!-- https://cogito.iot.linkeddata.es/def/process#Process -->


    <owl:Class rdf:about="https://cogito.iot.linkeddata.es/def/process#Process">
        <rdfs:comment>A series of actions aimed at accomplishing some result (in this case, related to a facility:Project)</rdfs:comment>
        <rdfs:label>Process</rdfs:label>
    </owl:Class>
    


    <!-- https://cogito.iot.linkeddata.es/def/process#ResourceTypeRequirement -->


    <owl:Class rdf:about="https://cogito.iot.linkeddata.es/def/process#ResourceTypeRequirement">
        <rdfs:comment>An entity that includes the requitrments that a task has pertaining a resource type</rdfs:comment>
        <rdfs:label>Resource Type Requirement</rdfs:label>
    </owl:Class>
    


    <!-- https://cogito.iot.linkeddata.es/def/process#SatetyAddingTask -->


    <owl:Class rdf:about="https://cogito.iot.linkeddata.es/def/process#SatetyAddingTask">
        <rdfs:subClassOf rdf:resource="https://cogito.iot.linkeddata.es/def/process#Task"/>
        <rdfs:comment>A task related to the safety domain that adds elements</rdfs:comment>
        <rdfs:label>Safety Adding Task</rdfs:label>
    </owl:Class>
    


    <!-- https://cogito.iot.linkeddata.es/def/process#SatetyRemovingTask -->


    <owl:Class rdf:about="https://cogito.iot.linkeddata.es/def/process#SatetyRemovingTask">
        <rdfs:subClassOf rdf:resource="https://cogito.iot.linkeddata.es/def/process#Task"/>
        <rdfs:comment>A task related to the safety domain that removes elements</rdfs:comment>
        <rdfs:label>Safety Removing Task</rdfs:label>
    </owl:Class>
    


    <!-- https://cogito.iot.linkeddata.es/def/process#Task -->


    <owl:Class rdf:about="https://cogito.iot.linkeddata.es/def/process#Task">
        <rdfs:comment>A piece of work, which is performed in a process:Process</rdfs:comment>
        <rdfs:label>Task</rdfs:label>
    </owl:Class>
    


    <!-- https://cogito.iot.linkeddata.es/def/process#UnitOfCurrency -->


    <owl:Class rdf:about="https://cogito.iot.linkeddata.es/def/process#UnitOfCurrency">
        <rdfs:comment>The currency used to measure a process:Cost</rdfs:comment>
        <rdfs:label>Unit of Currency</rdfs:label>
    </owl:Class>
    


    <!-- https://cogito.iot.linkeddata.es/def/process#VisualQualityTask -->


    <owl:Class rdf:about="https://cogito.iot.linkeddata.es/def/process#VisualQualityTask">
        <rdfs:subClassOf rdf:resource="https://cogito.iot.linkeddata.es/def/process#Task"/>
        <rdfs:comment>A task related to the visual quality domain</rdfs:comment>
        <rdfs:label>Visual Quality Task</rdfs:label>
    </owl:Class>
    


    <!-- https://cogito.iot.linkeddata.es/def/process#WorkOrder -->


    <owl:Class rdf:about="https://cogito.iot.linkeddata.es/def/process#WorkOrder">
        <rdfs:comment>A command or instruction authorizing specific work, repairs, etc., to be done</rdfs:comment>
        <rdfs:label>Work Order</rdfs:label>
    </owl:Class>
    


    <!-- https://cogito.iot.linkeddata.es/def/resource#Resource -->


    <owl:Class rdf:about="https://cogito.iot.linkeddata.es/def/resource#Resource">
        <rdfs:comment>A source of supply, support, or aid, especially one that can be readily drawn upon when needed</rdfs:comment>
        <rdfs:label>Resource</rdfs:label>
    </owl:Class>
    


    <!-- https://cogito.iot.linkeddata.es/def/resource#ResourceType -->


    <owl:Class rdf:about="https://cogito.iot.linkeddata.es/def/resource#ResourceType">
        <rdfs:comment>The kind of resources assigned to a process:Task or involved in a process:Process</rdfs:comment>
        <rdfs:label>Resource Type</rdfs:label>
    </owl:Class>
    


    <!-- https://cogito.iot.linkeddata.es/def/resource#Worker -->


    <owl:Class rdf:about="https://cogito.iot.linkeddata.es/def/resource#Worker">
        <rdfs:subClassOf rdf:resource="https://cogito.iot.linkeddata.es/def/resource#Resource"/>
        <rdfs:comment>A human resource that works in a project (especially performing a process:Task)</rdfs:comment>
        <rdfs:label>Worker</rdfs:label>
    </owl:Class>
</rdf:RDF>



<!-- Generated by the OWL API (version 5.1.14) https://github.com/owlcs/owlapi/ -->


