@prefix : <https://cogito.iot.linkeddata.es/def/iot#> .
@prefix owl: <http://www.w3.org/2002/07/owl#> .
@prefix rdf: <http://www.w3.org/1999/02/22-rdf-syntax-ns#> .
@prefix xml: <http://www.w3.org/XML/1998/namespace> .
@prefix xsd: <http://www.w3.org/2001/XMLSchema#> .
@prefix rdfs: <http://www.w3.org/2000/01/rdf-schema#> .
@base <https://cogito.iot.linkeddata.es/def/iot#> .

<https://cogito.iot.linkeddata.es/def/iot#> rdf:type owl:Ontology ;
                                             <http://purl.org/dc/elements/1.1/creator> "María Poveda Villalón" ,
                                                                                       "Raúl García Castro" ,
                                                                                       "Socorro  Bernardos Galindo" ;
                                             <http://purl.org/dc/elements/1.1/description> "The COGITO IoT ontology aims at modelling IoT devices and their measurements in the construction domain." ;
                                             <http://purl.org/dc/elements/1.1/title> "IoT ontology" ;
                                             <http://purl.org/dc/terms/license> <http://purl.org/NET/rdflicense/cc-by4.0> ;
                                             owl:versionInfo "0.5.0" .

#################################################################
#    Annotation properties
#################################################################

###  http://purl.org/dc/elements/1.1/creator
<http://purl.org/dc/elements/1.1/creator> rdf:type owl:AnnotationProperty .


###  http://purl.org/dc/elements/1.1/description
<http://purl.org/dc/elements/1.1/description> rdf:type owl:AnnotationProperty .


###  http://purl.org/dc/elements/1.1/title
<http://purl.org/dc/elements/1.1/title> rdf:type owl:AnnotationProperty .


###  http://purl.org/dc/terms/license
<http://purl.org/dc/terms/license> rdf:type owl:AnnotationProperty .


#################################################################
#    Object Properties
#################################################################

###  https://cogito.iot.linkeddata.es/def/iot#belongsToTagGroup
:belongsToTagGroup rdf:type owl:ObjectProperty ;
                   rdfs:range :TrackingTagGroup ;
                   rdfs:comment "Property relating an entity (especially an iot:TrackingTag) to an iot:TrackingTagGroup" ;
                   rdfs:label "belongs to tag group" .


###  https://cogito.iot.linkeddata.es/def/iot#hasLocation
:hasLocation rdf:type owl:ObjectProperty ;
             rdfs:comment "Property that relates an entity (especially a saref:Measurement) to the geo:Point it is located at" ;
             rdfs:label "has location" .


###  https://cogito.iot.linkeddata.es/def/iot#hasLocationKF
:hasLocationKF rdf:type owl:ObjectProperty ;
               rdfs:comment "Property that relates an entity (especially a saref:Measurement) to the geo:Point it is located at using a KF transformation" ;
               rdfs:label "has location KF" .


###  https://cogito.iot.linkeddata.es/def/iot#hasLocationMA
:hasLocationMA rdf:type owl:ObjectProperty ;
               rdfs:comment "Property that relates an entity (especially a saref:Measurement) to the geo:Point it is located at using a MA transformation" ;
               rdfs:label "has location MA" .


###  https://cogito.iot.linkeddata.es/def/iot#measuresLocation
:measuresLocation rdf:type owl:ObjectProperty ;
                  rdfs:subPropertyOf <https://saref.etsi.org/core#makesMeasurement> ;
                  rdfs:range :LocationMeasurement ;
                  rdfs:comment "Property relating an entity (especially an iot:TrackingTag) to an iot:LocationMeasurement" ;
                  rdfs:label "measures location" .


###  https://saref.etsi.org/core#isMeasurementOf
<https://saref.etsi.org/core#isMeasurementOf> rdf:type owl:ObjectProperty ;
                                              rdfs:isDefinedBy <https://saref.etsi.org/core#> ;
                                              rdfs:label "is measurement of" .


###  https://saref.etsi.org/core#makesMeasurement
<https://saref.etsi.org/core#makesMeasurement> rdf:type owl:ObjectProperty ;
                                               rdfs:isDefinedBy <https://saref.etsi.org/core#> ;
                                               rdfs:label "makes measurement" .


#################################################################
#    Data properties
#################################################################

###  http://purl.org/dc/terms/identifier
<http://purl.org/dc/terms/identifier> rdf:type owl:DatatypeProperty ;
                                      rdfs:isDefinedBy <http://purl.org/dc/terms/> ;
                                      rdfs:label "identifier" .


###  http://purl.org/dc/terms/titile
<http://purl.org/dc/terms/titile> rdf:type owl:DatatypeProperty ;
                                  rdfs:isDefinedBy <http://purl.org/dc/terms/> ;
                                  rdfs:label "title" .


###  https://cogito.iot.linkeddata.es/def/iot#coordX
:coordX rdf:type owl:DatatypeProperty ;
        rdfs:comment "Property referring to the coordinate x of a location measured by a tracking tag" ;
        rdfs:label "coordinate x" .


###  https://cogito.iot.linkeddata.es/def/iot#coordY
:coordY rdf:type owl:DatatypeProperty ;
        rdfs:comment "Property referring to the coordinate y of a location measured by a tracking tag" ;
        rdfs:label "coordinate y" .


###  https://cogito.iot.linkeddata.es/def/iot#coordZ
:coordZ rdf:type owl:DatatypeProperty ;
        rdfs:comment "Property referring to the coordinate z of a location measured by a tracking tag" ;
        rdfs:label "coordinate z" .


###  https://cogito.iot.linkeddata.es/def/iot#inferredAccuracy
:inferredAccuracy rdf:type owl:DatatypeProperty ;
                  rdfs:comment "Property referring to the accuracy of a location measured by  a tracking tag" ;
                  rdfs:label "inferred accuracy" .


###  https://cogito.iot.linkeddata.es/def/iot#inferredMovement
:inferredMovement rdf:type owl:DatatypeProperty ;
                  rdfs:comment "Property referring to the movement  associated to a location measured by a tracking tag" ;
                  rdfs:label "inferred movement" .


###  https://cogito.iot.linkeddata.es/def/iot#inferredSpeed
:inferredSpeed rdf:type owl:DatatypeProperty ;
               rdfs:comment "Property referring to the speed  associated to a location measured by a tracking tag" ;
               rdfs:label "inferred speed" .


###  https://cogito.iot.linkeddata.es/def/iot#locationRadius
:locationRadius rdf:type owl:DatatypeProperty ;
                rdfs:comment "Property referring to the location radius associated to a location measured by a tracking tag" ;
                rdfs:label "location radius" .


###  https://saref.etsi.org/core#hasTimestamp
<https://saref.etsi.org/core#hasTimestamp> rdf:type owl:DatatypeProperty ;
                                           rdfs:comment "has timestamp" ;
                                           rdfs:isDefinedBy <https://saref.etsi.org/core#> .


#################################################################
#    Classes
#################################################################

###  http://www.opengis.net/ont/sfl#Point
<http://www.opengis.net/ont/sfl#Point> rdf:type owl:Class ;
                                       rdfs:isDefinedBy <http://www.opengis.net/ont/geosparq#> ;
                                       rdfs:label "Point" .


###  https://cogito.iot.linkeddata.es/def/facility#SpatialZone
<https://cogito.iot.linkeddata.es/def/facility#SpatialZone> rdf:type owl:Class ;
                                                            rdfs:comment "A subclass of bot:Zone and, as such, a part of the physical or a virtual world that is inherently both located in this world and has a 3D spatial extent." ;
                                                            rdfs:label "Spatial Zone" .


###  https://cogito.iot.linkeddata.es/def/iot#EquipmentTagGroup
:EquipmentTagGroup rdf:type owl:Class ;
                   rdfs:subClassOf :TrackingTagGroup ;
                   rdfs:comment "A tracking tag group belonging to a piece of equipment" ;
                   rdfs:label "Equipment Tag Group" .


###  https://cogito.iot.linkeddata.es/def/iot#HumanTagGroup
:HumanTagGroup rdf:type owl:Class ;
               rdfs:subClassOf :TrackingTagGroup ;
               rdfs:comment "A tracking tag group belonging to a human" ;
               rdfs:label "Human Tag Group" .


###  https://cogito.iot.linkeddata.es/def/iot#LocationMeasurement
:LocationMeasurement rdf:type owl:Class ;
                     rdfs:subClassOf <https://saref.etsi.org/core/Measurement> ;
                     rdfs:comment "The location measured by an entity (especially an iot:TrackingTag)" ;
                     rdfs:label "Location Measurement" .


###  https://cogito.iot.linkeddata.es/def/iot#TrackedZone
:TrackedZone rdf:type owl:Class ;
             rdfs:subClassOf <https://cogito.iot.linkeddata.es/def/facility#SpatialZone> ;
             rdfs:comment "An entity used to represent zones used by the IoT preprocessing module" ;
             rdfs:label "Tracked Zone" .


###  https://cogito.iot.linkeddata.es/def/iot#TrackingTag
:TrackingTag rdf:type owl:Class ;
             rdfs:subClassOf <https://saref.etsi.org/core/Device> ;
             rdfs:comment "A subclass of saref:Device and, as such, a tangible object designed to accomplish a particular task; in this case signalling its location" ,
                          "An entity" ;
             rdfs:label "Tracking Tag" .


###  https://cogito.iot.linkeddata.es/def/iot#TrackingTagGroup
:TrackingTagGroup rdf:type owl:Class ;
                  rdfs:comment "An entity used to group tracking tags" ;
                  rdfs:label "Tracking Tag Group" .


###  https://cogito.iot.linkeddata.es/def/resource#Resource
<https://cogito.iot.linkeddata.es/def/resource#Resource> rdf:type owl:Class ;
                                                         rdfs:subClassOf <https://saref.etsi.org/core/FeatureOfInterest> ;
                                                         rdfs:comment "A source of supply, support, or aid, especially one that can be readily drawn upon when needed; and from which a property is measured" .


###  https://saref.etsi.org/core/Device
<https://saref.etsi.org/core/Device> rdf:type owl:Class ;
                                     rdfs:isDefinedBy <https://saref.etsi.org/core#> ;
                                     rdfs:label "Device" .


###  https://saref.etsi.org/core/FeatureOfInterest
<https://saref.etsi.org/core/FeatureOfInterest> rdf:type owl:Class ;
                                                rdfs:isDefinedBy <https://saref.etsi.org/core#> ;
                                                rdfs:label "Feature of Interest" .


###  https://saref.etsi.org/core/Measurement
<https://saref.etsi.org/core/Measurement> rdf:type owl:Class ;
                                          rdfs:isDefinedBy <https://saref.etsi.org/core#> ;
                                          rdfs:label "Measurement" .


###  Generated by the OWL API (version 5.1.14) https://github.com/owlcs/owlapi/
